implemented RankAux

thys/MFODL_Monitor_Devel/Optimized_Agg.thy
@@ -1,13 +1,45 @@
 theory Optimized_Agg
   imports Monitor
+  Ordered_Statistics_Tree
 begin
+
+
+fun less_eq_event_data' where
+  "less_eq_event_data' (EInt x) (EInt y) \<longleftrightarrow> x \<le> y"
+| "less_eq_event_data' (EInt _) _ \<longleftrightarrow> True"
+| "less_eq_event_data' (EFloat _) (EInt _) \<longleftrightarrow> False"
+| "less_eq_event_data' (EFloat x) (EFloat y) \<longleftrightarrow> lle_double x y"
+| "less_eq_event_data' (EFloat _) (EString _) \<longleftrightarrow> True"
+| "less_eq_event_data' (EString x) (EString y) \<longleftrightarrow> x \<le> y"
+| "less_eq_event_data' (EString _) _ \<longleftrightarrow> False"
+
+fun less_event_data' :: "event_data \<Rightarrow> event_data \<Rightarrow> bool"  where
+  "less_event_data' (EFloat x) (EFloat y) \<longleftrightarrow> lless_double x y" |
+  "less_event_data' x y \<longleftrightarrow> less_eq_event_data' x y \<and> \<not> (y = x)"
+
+lemma lin1: "less_event_data' x y = (less_eq_event_data' x y \<and> \<not> less_eq_event_data' y x)"
+proof(cases x)
+case (EInt x1) then show ?thesis by (cases y) auto
+next case (EFloat x2) then show ?thesis by (cases y) auto
+next case (EString x3) then show ?thesis by (cases y) auto
+qed
+
+lemma lin2: "less_eq_event_data' x x"
+  by(cases x) auto
+
+interpretation event_data_linorder : linorder less_eq_event_data' less_event_data'
+  using lin1 lin2  sorry
+
+instantiation event_data :: linorder 
+begin
+instance sorry
+end
 
 type_synonym 'a agg_map = "(event_data tuple, 'a) mapping"
 
-datatype aggaux' = CntAux nat
-
-datatype aggaux = CntAux "nat agg_map" | SumAux "(nat \<times> event_data) agg_map" | MinAux "event_data table"
-  | MaxAux "event_data table" | MedAux "event_data table"
+datatype aggaux = CntAux "nat agg_map" | 
+                  SumAux "(nat \<times> event_data) agg_map" | 
+                  RankAux "(event_data wbt) agg_map"
 
 definition group where [simp]:
   "group k b X = Set.filter (\<lambda>x. drop b x = k) X"
@@ -16,12 +48,17 @@ definition group_multiset where [simp]:
   "group_multiset k b f X = (let group = group k b X in
                       (\<lambda>y. (y, ecard (Set.filter (\<lambda>x. meval_trm f x = y) group))) ` meval_trm f ` group)"
 
+definition valid_finite_mset where
+  "valid_finite_mset X = ((\<forall>k x y. x \<noteq> y \<and> (k, x) \<in> X \<longrightarrow> (k, y) \<notin> X) \<and> 
+                              (\<forall>k x. (k, x) \<in> X \<longrightarrow> x \<noteq> \<infinity>))"
 
-definition valid_aggmap :: "(event_data list \<Rightarrow> 'a) \<Rightarrow> nat \<Rightarrow> Formula.trm \<Rightarrow> (event_data option list, 'a) mapping \<Rightarrow> event_data option list set \<Rightarrow> bool" where [simp]:
-  "valid_aggmap g b f m X \<longleftrightarrow> (\<forall>k. k \<in> (drop b) ` X \<longleftrightarrow> k \<in> Mapping.keys m) \<and>
-                    (\<forall>k. k \<in> Mapping.keys m \<longrightarrow> Mapping.lookup m k = 
-                    (let M = group_multiset k b f X
-                    in Some (g (flatten_multiset M))))"
+fun mset_conv :: "(event_data \<times> enat) set  \<Rightarrow> event_data multiset" where
+  "mset_conv s = Finite_Set.fold (\<lambda> (t, m) b. (replicate_mset (the_enat m) t) + b) {#} s"
+
+definition valid_aggmap :: "('a option \<Rightarrow> (event_data \<times> enat) set \<Rightarrow>  bool) \<Rightarrow> nat \<Rightarrow> Formula.trm \<Rightarrow> (event_data option list, 'a) mapping \<Rightarrow> event_data option list set \<Rightarrow> bool" where [simp]:
+  "valid_aggmap P b f m X \<longleftrightarrow> (\<forall>k. k \<in> (drop b) ` X \<longleftrightarrow> k \<in> Mapping.keys m) \<and>
+                    (\<forall>k. k \<in> Mapping.keys m \<longrightarrow> (let M = group_multiset k b f X
+                    in P (Mapping.lookup m k) M))"
 
 fun valid_maggaux :: "aggargs \<Rightarrow> aggaux \<Rightarrow> event_data table \<Rightarrow> bool" where
   "valid_maggaux \<lparr>aggargs_cols = cols, aggargs_n = n, aggargs_g0 = g0, aggargs_y = y, aggargs_\<omega> = \<omega>, aggargs_b = b, aggargs_f = f\<rparr> aux X = 
@@ -29,69 +66,86 @@ fun valid_maggaux :: "aggargs \<Rightarrow> aggaux \<Rightarrow> event_data tabl
   (let aggtype = fst \<omega> in case aux of 
       CntAux m \<Rightarrow>
         (aggtype = Formula.Agg_Cnt) \<and> 
-        (valid_aggmap (\<lambda>k. length k) b f m X)
+        (valid_aggmap (\<lambda>k s. 
+                      k = Some(length(flatten_multiset(s)))) 
+                      b f m X)
     | SumAux m \<Rightarrow> (aggtype = Formula.Agg_Sum \<or> aggtype = Formula.Agg_Avg) \<and> (type_restr \<lparr>aggargs_cols = cols, aggargs_n = n, aggargs_g0 = g0, aggargs_y = y, aggargs_\<omega> = \<omega>, aggargs_b = b, aggargs_f = f\<rparr> X) \<and>
                   (let y0 = (if aggtype = Formula.Agg_Sum then snd \<omega> else EInt 0) in
-                  (valid_aggmap (\<lambda>k. (length k, foldl plus y0 k)) b f m X))
-    | MinAux t \<Rightarrow> (aggtype = Formula.Agg_Min) \<and> t = X
-    | MaxAux t \<Rightarrow> (aggtype = Formula.Agg_Max) \<and> t = X
-    | MedAux t \<Rightarrow> (aggtype = Formula.Agg_Med) \<and> t = X))"
+                  (valid_aggmap 
+                  (\<lambda>k s. k = Some(length(flatten_multiset(s)), foldl plus y0 (flatten_multiset s))) 
+                  b f m X))
+    | RankAux m \<Rightarrow> (aggtype = Formula.Agg_Min \<or> aggtype = Formula.Agg_Max \<or> aggtype = Formula.Agg_Med) \<and>
+                   valid_aggmap 
+                   (\<lambda>k s. (case k of Some(t) \<Rightarrow> valid_wbt_mset t (mset_conv s) |
+                                     None \<Rightarrow> False)) 
+                   b f m X))"
 
 fun init_maggaux :: "aggargs \<Rightarrow> aggaux" where
   "init_maggaux args =
   (let aggtype = fst (aggargs_\<omega> args) in case aggtype of
       Formula.Agg_Cnt \<Rightarrow> CntAux Mapping.empty
     | Formula.Agg_Sum \<Rightarrow> SumAux Mapping.empty
-    | Formula.Agg_Min \<Rightarrow> MinAux {}
-    | Formula.Agg_Max \<Rightarrow> MaxAux {}
+    | Formula.Agg_Min \<Rightarrow> RankAux Mapping.empty
+    | Formula.Agg_Max \<Rightarrow> RankAux Mapping.empty
     | Formula.Agg_Avg \<Rightarrow> SumAux Mapping.empty
-    | Formula.Agg_Med \<Rightarrow> MedAux {})"
+    | Formula.Agg_Med \<Rightarrow> RankAux Mapping.empty)"
 
 fun insert_cnt :: "aggargs \<Rightarrow>  event_data tuple \<Rightarrow> nat agg_map \<Rightarrow> nat agg_map" where
   "insert_cnt args t m = (let group = drop (aggargs_b args) t 
-                       in case (Mapping.lookup m group) of
-                        Some i \<Rightarrow> Mapping.update group (i + 1) m
-                      | None \<Rightarrow> Mapping.update group 1 m)"
+                          in case (Mapping.lookup m group) of
+                            Some i \<Rightarrow> Mapping.update group (i + 1) m |
+                            None \<Rightarrow> Mapping.update group 1 m)"
 
 fun insert_sum :: "aggargs \<Rightarrow> event_data tuple \<Rightarrow> (nat \<times> event_data) agg_map \<Rightarrow> (nat \<times> event_data) agg_map" where
   "insert_sum args t m = (let group = drop (aggargs_b args) t;
                               aggtype = fst (aggargs_\<omega> args);
                               y0 = (if aggtype = Formula.Agg_Sum then snd (aggargs_\<omega> args) else EInt 0);
-                                         term = meval_trm (aggargs_f args) t
-                                     in case (Mapping.lookup m group) of
-                        Some (cnt, agg_sum) \<Rightarrow> Mapping.update group (cnt + 1, agg_sum + term) m
-                      | None \<Rightarrow> Mapping.update group (1, y0 + term) m)"
+                              term = meval_trm (aggargs_f args) t
+                          in case (Mapping.lookup m group) of
+                            Some (cnt, agg_sum) \<Rightarrow> Mapping.update group (cnt + 1, agg_sum + term) m |
+                            None \<Rightarrow> Mapping.update group (1, y0 + term) m)"
+
+fun insert_rank :: "aggargs \<Rightarrow> event_data tuple \<Rightarrow> (event_data wbt) agg_map \<Rightarrow> (event_data wbt) agg_map" where
+  "insert_rank args t m = (let group = drop (aggargs_b args) t;
+                               term = meval_trm (aggargs_f args) t
+                           in case (Mapping.lookup m group) of
+                            Some t \<Rightarrow> Mapping.update group (insert term t) m |
+                            None \<Rightarrow> Mapping.update group (insert term Leaf) m)"
 
 fun insert_maggaux :: "aggargs \<Rightarrow> event_data table \<Rightarrow> aggaux \<Rightarrow> aggaux" where
   "insert_maggaux args data aux = (case aux of
     CntAux m \<Rightarrow> CntAux (Finite_Set.fold (insert_cnt args) m data)
   | SumAux m \<Rightarrow> SumAux (Finite_Set.fold (insert_sum args) m data)
-  | MinAux t \<Rightarrow> MinAux (t \<union> data)
-  | MaxAux t \<Rightarrow> MaxAux (t \<union> data)
-  | MedAux t \<Rightarrow> MedAux (t \<union> data))"
+  | RankAux m \<Rightarrow> RankAux (Finite_Set.fold (insert_rank args) m data))"
 
-fun delete_cnt :: "nat \<Rightarrow> nat agg_map \<Rightarrow> event_data tuple \<Rightarrow> nat agg_map" where
-  "delete_cnt b m t = (let group = drop b t
+fun delete_cnt :: "aggargs \<Rightarrow> event_data tuple \<Rightarrow> nat agg_map \<Rightarrow> nat agg_map" where
+  "delete_cnt args t m = (let group = drop (aggargs_b args) t
                        in case (Mapping.lookup m group) of
                          Some i \<Rightarrow> (if i = 1 then Mapping.delete group m 
                                     else Mapping.update group (i - 1) m)
                        | None \<Rightarrow> m)"
 
-fun delete_sum :: "aggargs \<Rightarrow> (nat \<times> event_data) agg_map \<Rightarrow> event_data tuple \<Rightarrow> (nat \<times> event_data) agg_map" where
-  "delete_sum args m t = (let group = drop (aggargs_b args) t;
+fun delete_sum :: "aggargs \<Rightarrow> event_data tuple \<Rightarrow> (nat \<times> event_data) agg_map \<Rightarrow> (nat \<times> event_data) agg_map" where
+  "delete_sum args t m = (let group = drop (aggargs_b args) t;
                               term = meval_trm (aggargs_f args) t
                           in case (Mapping.lookup m group) of
                             Some (cnt, agg_sum) \<Rightarrow> (if cnt = 1 then Mapping.delete group m
                                                     else Mapping.update group (cnt - 1, agg_sum - term) m)
                           | None \<Rightarrow> m)"
 
+fun delete_rank :: "aggargs \<Rightarrow> event_data tuple \<Rightarrow> (event_data wbt) agg_map \<Rightarrow> (event_data wbt) agg_map" where
+  "delete_rank args t m = (let group = drop (aggargs_b args) t;
+                               term = meval_trm (aggargs_f args) t
+                           in case (Mapping.lookup m group) of
+                            Some (Node Leaf _ Leaf) \<Rightarrow> Mapping.delete group m |
+                            Some t \<Rightarrow> Mapping.update group (delete term t) m |
+                            None \<Rightarrow> m)"
+
 fun delete_maggaux :: "aggargs \<Rightarrow> event_data table \<Rightarrow> aggaux \<Rightarrow> aggaux" where
   "delete_maggaux args data aux = (case aux of
-    CntAux m \<Rightarrow> CntAux (foldl (delete_cnt (aggargs_b args)) m (csorted_list_of_set data))
-  | SumAux m \<Rightarrow> SumAux (foldl (delete_sum args) m (csorted_list_of_set data))
-  | MinAux t \<Rightarrow> MinAux (t - data)
-  | MaxAux t \<Rightarrow> MaxAux (t - data)
-  | MedAux t \<Rightarrow> MedAux (t - data))"
+    CntAux m \<Rightarrow> CntAux (Finite_Set.fold (delete_cnt args) m data)
+  | SumAux m \<Rightarrow> SumAux (Finite_Set.fold (delete_sum args) m data)
+  | RankAux m \<Rightarrow> RankAux (Finite_Set.fold (delete_rank args) m data))"
 
 fun result_maggaux :: "aggargs \<Rightarrow> aggaux \<Rightarrow> event_data table" where
   "result_maggaux \<lparr>aggargs_cols = cols, aggargs_n = n, aggargs_g0 = g0, aggargs_y = y, aggargs_\<omega> = \<omega>, aggargs_b = b, aggargs_f = f\<rparr> aux = (case aux of
@@ -109,9 +163,23 @@ fun result_maggaux :: "aggargs \<Rightarrow> aggaux \<Rightarrow> event_data tab
                       else (\<lambda>k. (case Mapping.lookup m k of
                                    Some (cnt, agg_sum) \<Rightarrow> k[y:=Some (EFloat ((double_of_event_data agg_sum) / (double_of_int cnt)))] 
                                  | None \<Rightarrow> k)) ` Mapping.keys m)
-  | MinAux t \<Rightarrow> eval_aggargs \<lparr>aggargs_cols = cols, aggargs_n = n, aggargs_g0 = g0, aggargs_y = y, aggargs_\<omega> = \<omega>, aggargs_b = b, aggargs_f = f\<rparr> t
-  | MaxAux t \<Rightarrow> eval_aggargs \<lparr>aggargs_cols = cols, aggargs_n = n, aggargs_g0 = g0, aggargs_y = y, aggargs_\<omega> = \<omega>, aggargs_b = b, aggargs_f = f\<rparr> t
-  | MedAux t \<Rightarrow> eval_aggargs \<lparr>aggargs_cols = cols, aggargs_n = n, aggargs_g0 = g0, aggargs_y = y, aggargs_\<omega> = \<omega>, aggargs_b = b, aggargs_f = f\<rparr> t)"
+  | RankAux m \<Rightarrow> (if g0 \<and> Mapping.keys m = {}
+                      then singleton_table n y (eval_agg_op \<omega> {})
+                      else if fst \<omega> = Formula.Agg_Min
+                      then (\<lambda>k. (case Mapping.lookup m k of 
+                                   Some t \<Rightarrow> k[y:=Some (select t 0)]
+                                 | None \<Rightarrow> k)) ` Mapping.keys m
+                      else if fst \<omega> = Formula.Agg_Max
+                      then (\<lambda>k. (case Mapping.lookup m k of
+                                   Some t \<Rightarrow> k[y:=Some (select t (size t - 1))]
+                                 | None \<Rightarrow> k)) ` Mapping.keys m
+                      else (\<lambda>k. (case Mapping.lookup m k of
+                                   Some t \<Rightarrow> (let u = size t;
+                                              u' = u div 2;
+      aggval = (if even u then (double_of_event_data (select t (u' - 1)) + double_of_event_data (select t u') / double_of_int 2)
+                          else double_of_event_data (select t u')) in
+                                              k[y:=Some (EFloat aggval)])
+                                 | None \<Rightarrow> k)) ` Mapping.keys m))"
 
 fun plus' :: "event_data \<Rightarrow> event_data \<Rightarrow> event_data" where
   "plus' (EInt x) (EInt y) = EInt (x + y)"
@@ -120,6 +188,7 @@ fun plus' :: "event_data \<Rightarrow> event_data \<Rightarrow> event_data" wher
 fun minus' :: "event_data \<Rightarrow> event_data \<Rightarrow> event_data" where
   "minus' (EInt x) (EInt y) = EInt (y - x)"
 | "minus' (_::event_data) _ = EFloat nan"
+
 
 lemma iter_plus'_int: 
   assumes "t \<in> range EInt" and "y \<in> range EInt"
@@ -143,14 +212,43 @@ next
   then show ?case using assms Suc by auto
 qed
 
+lemma plus'_minus'_comm': 
+  assumes "y0 \<in> range EInt" and "t \<in> range EInt"
+  shows "(plus' t ^^ n) (minus' t y0)  = minus' t ((plus' t ^^ n) y0)"
+proof(induction n)
+case 0
+  then show ?case by auto
+next
+  case (Suc n)
+  have "(plus' t ^^ n) y0 \<in> range EInt" using iter_plus'_int assms by auto
+  then show ?case using assms Suc by auto
+qed
+
 lemma plus'_minus'_id:
   assumes "t \<in> range EInt" and "y0 \<in> range EInt"
   shows "((minus' t) ^^ n \<circ> (plus' t) ^^ n) y0 = y0"
   using Suc plus'_minus'_comm iter_plus'_int assms by (induction n) auto
 
+lemma plus'_minus'_minus:
+  assumes "t \<in> range EInt" and "y0 \<in> range EInt"
+  shows "((plus' t) ^^ i \<circ> ((minus' t) ^^ (i + 1))) y0 = minus' t y0"
+proof(induction i)
+case 0
+  then show ?case by auto
+next
+  case (Suc i)
+  have "minus' t ((minus' t ^^ i) y0) \<in> range EInt" using assms iter_minus'_int by(auto simp: funpow_swap1)
+  then show ?case using plus'_minus'_comm' assms  Suc by(auto) 
+qed
+
 lemma plus_plus'_equiv:
   assumes "x \<in> range EInt" and "y \<in> range EInt"
   shows "plus x y = plus' x y"
+  using assms by auto
+
+lemma minus_minus'_equiv:
+  assumes "x \<in> range EInt" and "y \<in> range EInt"
+  shows "minus x y = minus' y x"
   using assms by auto
 
 lemma plus'_aux: "\<And>y x. plus' y \<circ> plus' x = plus' x \<circ> plus' y"
@@ -190,10 +288,50 @@ proof
     then show ?thesis by auto
   qed
 qed
-    
+
+lemma minus'_aux: "\<And>y x. minus' y \<circ> minus' x = minus' x \<circ> minus' y"
+proof
+  fix xa x y
+  show "(minus' y \<circ> minus' x) xa = (minus' x \<circ> minus' y) xa"
+  proof(cases xa)
+    case (EInt x1)
+    then have xa_int: "xa = EInt x1" by auto
+    then show ?thesis
+    proof(cases x)
+      case (EInt x1)
+      then have x_int: "x = EInt x1" by auto
+      then show ?thesis
+      proof(cases y)
+        case (EInt x1)
+        then show ?thesis using xa_int x_int by auto
+      next
+        case (EFloat x2)
+        then show ?thesis by auto
+      next
+        case (EString x3)
+        then show ?thesis by auto
+      qed
+    next
+      case (EFloat x2)
+      then show ?thesis by auto
+    next
+      case (EString x3)
+      then show ?thesis by auto
+    qed
+  next
+    case (EFloat x2)
+    then show ?thesis by auto
+  next
+    case (EString x3)
+    then show ?thesis by auto
+  qed
+qed
 
 lemma comp_fun_commute_plus': "comp_fun_commute plus'"
   using plus'_aux by(unfold_locales) auto
+
+lemma comp_fun_commute_minus': "comp_fun_commute minus'"
+  using minus'_aux by(unfold_locales) auto
 
 lemma comm_plus': "plus' x y = plus' y x"
   by (smt (verit, best) add.commute plus'.elims plus'.simps(1))
@@ -202,8 +340,8 @@ lemma unique_term_multiset: "(t, y1) \<in> group_multiset k b f X \<Longrightarr
 proof rule
   assume term_in: "(t, y1) \<in> group_multiset k b f X" and not_eq: "y2 \<noteq> y1" and term_in_2: "(t, y2) \<in> group_multiset k b f X"
   define group where [simp]: "group = Set.filter (\<lambda>x. drop b x = k) X"
-  have "y2 = ecard (Set.filter (\<lambda>x. meval_trm f x = t) group)" using term_in_2 by(auto simp: Let_def)
-  moreover have "y1 = ecard (Set.filter (\<lambda>x. meval_trm f x = t) group)" using term_in by(auto simp: Let_def)
+  have "y2 = ecard (Set.filter (\<lambda>x. meval_trm f x = t) group)" using term_in_2 by auto
+  moreover have "y1 = ecard (Set.filter (\<lambda>x. meval_trm f x = t) group)" using term_in by auto
   ultimately show False using not_eq by auto
 qed
 
@@ -211,7 +349,7 @@ lemma valid_init_maggaux_unfolded: "safe_aggargs \<lparr>aggargs_cols = cols, ag
   (*by (cases "fst \<omega>") (auto simp: type_restr_def Let_def)*)
   sorry
 
-lemma valid_init_maggaux: "safe_aggargs args \<Longrightarrow> valid_maggaux args (init_maggaux args) {}"
+lemma valid_init_maggaux': "safe_aggargs args \<Longrightarrow> valid_maggaux args (init_maggaux args) {}"
   using valid_init_maggaux_unfolded by (cases args) fast
 
 definition valid_sumaux_maps where "valid_sumaux_maps = {m::(nat \<times> event_data) agg_map. \<forall>k a b. Mapping.lookup m k = Some (a, b) \<longrightarrow> b \<in> range EInt}"
@@ -224,6 +362,14 @@ fun insert_sum_comm :: "aggargs \<Rightarrow> event_data tuple \<Rightarrow> (na
                         (if term \<in> range EInt then (case (Mapping.lookup m group) of
                         Some (cnt, agg_sum) \<Rightarrow> Mapping.update group (cnt + 1, plus' term agg_sum) m
                       | None \<Rightarrow> Mapping.update group (1, plus' y0 term) m) else m))"
+
+fun delete_sum_comm :: "aggargs \<Rightarrow> event_data tuple \<Rightarrow> (nat \<times> event_data) agg_map \<Rightarrow> (nat \<times> event_data) agg_map" where
+  "delete_sum_comm args t m = (let group = drop (aggargs_b args) t;
+                              term = meval_trm (aggargs_f args) t in 
+                           (if term \<in> range EInt then (case (Mapping.lookup m group) of
+                            Some (cnt, agg_sum) \<Rightarrow> (if cnt = 1 then Mapping.delete group m
+                                                    else Mapping.update group (cnt - 1, minus' term agg_sum) m)
+                          | None \<Rightarrow> m) else m))"
 
 lemma flatten_multiset_eint:
   assumes "\<And> t m. (t, m) \<in> M \<Longrightarrow> t \<in> range EInt"
@@ -253,15 +399,15 @@ proof -
     define M where "M = flatten_multiset(group_multiset k b f X)"
     have "k \<in> Mapping.keys m" by (simp add: assm keys_is_none_rep)
     then have s_def: "s = foldl (+) y0 (M)" 
-      using assms y0_def assm by(auto simp:Let_def M_def)
+      using assms y0_def assm by(auto simp: M_def)
     have "\<And>t m. (t, m) \<in> group_multiset k b f X \<Longrightarrow> t \<in> range EInt"
-      using assms by(auto simp:Let_def type_restr_def image_subset_iff)
+      using assms by(auto simp: type_restr_def image_subset_iff)
     moreover have "finite (group_multiset k b f X)"
-      using assms by(simp add:Let_def)
+      using assms by simp
     ultimately have "set(M) \<subseteq> range EInt"
       using flatten_multiset_eint by (auto simp:M_def)
     moreover have "y0 \<in> range EInt" using assms
-      by(auto simp:y0_def type_restr_def Let_def)
+      by(auto simp:y0_def type_restr_def)
     ultimately show "s \<in> range EInt" using s_def
       by(induction M arbitrary: y0) auto
   qed
@@ -273,13 +419,33 @@ lemma insert_sum_equiv:
   and "snd (aggargs_\<omega> args) \<in> range EInt"
   and "m \<in> valid_sumaux_maps"
   shows "insert_sum args t m = insert_sum_comm args t m"
-  using assms plus_plus'_equiv comm_plus' by (auto simp:Let_def valid_sumaux_maps_def split:option.splits) 
+  using assms plus_plus'_equiv comm_plus' by (auto simp: valid_sumaux_maps_def split:option.splits) 
+
+lemma delete_sum_equiv:
+  assumes "meval_trm (aggargs_f args) t \<in> range EInt"
+  and "snd (aggargs_\<omega> args) \<in> range EInt"
+  and "m \<in> valid_sumaux_maps"
+  shows "delete_sum args t m = delete_sum_comm args t m"
+  using assms minus_minus'_equiv comm_plus' by (auto simp: valid_sumaux_maps_def split:option.splits) 
 
 lemma insert_sum_comm: "(insert_sum_comm args x \<circ> insert_sum_comm args y) m  = (insert_sum_comm args y \<circ> insert_sum_comm args x) m"
-  using comm_plus' comp_fun_commute_plus' comp_fun_commute.fun_left_comm[of plus'] by(auto split:option.splits simp add: Let_def update_update lookup_update')
+  unfolding insert_sum_comm.simps Let_def
+  using comp_fun_commute_plus' comp_fun_commute.fun_left_comm[of plus'] comm_plus'
+  by(transfer) (auto split:option.splits)
 
 lemma insert_cnt_comm: "(insert_cnt args x \<circ> insert_cnt args y) m  = (insert_cnt args y \<circ> insert_cnt args x) m"
-  by (auto split:option.splits simp add: Let_def update_update(2) lookup_update') 
+  unfolding insert_cnt.simps Let_def by(transfer) (auto split:option.splits)
+
+
+lemma delete_sum_comm: "(delete_sum_comm args x \<circ> delete_sum_comm args y) m  = (delete_sum_comm args y \<circ> delete_sum_comm args x) m"
+  unfolding delete_sum_comm.simps Let_def
+  using comp_fun_commute_minus' comp_fun_commute.fun_left_comm[of minus'] 
+  by(transfer) (auto split:option.splits)
+
+lemma delete_cnt_comm: "(delete_cnt args x \<circ> delete_cnt args y) m  = (delete_cnt args y \<circ> delete_cnt args x) m"
+  unfolding delete_cnt.simps Let_def
+  by(transfer) (auto split:option.splits)
+
 
 lemma cmp_comm: 
   assumes commute_f: "comp_fun_commute f"
@@ -366,53 +532,46 @@ lemma foldl_flatten_multiset:
 lemma length_fold: "length xs = fold (\<lambda> _ n. n + 1) xs 0"
   by (induction xs) (auto simp:fold_commute_apply)
 
-lemma plus'_iter_one: "((plus') (meval_trm f elem) ^^ 1) = (plus') (meval_trm f elem)"
-  by auto
-
 lemma plus'_iter_one_enat: "((plus') (meval_trm f elem) ^^ the_enat 1) = (plus') (meval_trm f elem)"
-  using plus'_iter_one by (simp add: enat_defs(2))
-  
+  by (simp add: enat_defs(2))
 
-lemma length_flatten_multiset: 
-  assumes "finite M"
-  shows "length (flatten_multiset M) = Finite_Set.fold (\<lambda> (t, m) y. y + (the_enat m)) 0 M"
-  using length_fold[of "flatten_multiset M"] fold_flatten_multiset[of M "(\<lambda>_ n. n + 1)" 0]
-  by (simp add: fold_flatten_multiset assms comp_fun_commute.intro) (meson add.commute)
+lemma minus'_iter_one_enat: "((minus') (meval_trm f elem) ^^ the_enat 1) = (minus') (meval_trm f elem)"
+  by (simp add: enat_defs(2))
 
 lemma other_evals_unchanged:
   assumes elem_group: "drop b elem = k"
   and diff_group: "x \<noteq> meval_trm f elem"
-  shows "(x, y) \<in> group_multiset k b f (insert elem X) \<longleftrightarrow> (x, y) \<in> group_multiset k b f X"
+  shows "(x, y) \<in> group_multiset k b f (Set.insert elem X) \<longleftrightarrow> (x, y) \<in> group_multiset k b f X"
 proof
   define old_group where [simp]: "old_group = group k b X"
   define new_group where [simp]: "new_group = group k b (X \<union> {elem})"
   have aux1: "\<And>x. x \<noteq> meval_trm f elem \<Longrightarrow> Set.filter (\<lambda>xa. meval_trm f xa = x) new_group = Set.filter (\<lambda>xa. meval_trm f xa = x) old_group" by auto
-  assume assm: "(x, y) \<in> group_multiset k b f (insert elem X)"
-  then have x_old_eval: "x \<in> meval_trm f ` old_group" using diff_group by(auto simp: Let_def)
-  have "y = ecard (Set.filter (\<lambda>xa. meval_trm f xa = x) new_group)" using assm by(auto simp: Let_def)
+  assume assm: "(x, y) \<in> group_multiset k b f (Set.insert elem X)"
+  then have x_old_eval: "x \<in> meval_trm f ` old_group" using diff_group by auto
+  have "y = ecard (Set.filter (\<lambda>xa. meval_trm f xa = x) new_group)" using assm by auto
   then have "y =  ecard (Set.filter (\<lambda>xa. meval_trm f xa = x) old_group)" using aux1 diff_group by auto
-  then show "(x, y) \<in>  group_multiset k b f X" using x_old_eval by (auto simp: Let_def)
+  then show "(x, y) \<in>  group_multiset k b f X" using x_old_eval by auto
 next
   define old_group where [simp]: "old_group = group k b X"
   define new_group where [simp]: "new_group = group k b (X \<union> {elem})"
   have aux1: "\<And>x. x \<noteq> meval_trm f elem \<Longrightarrow> Set.filter (\<lambda>xa. meval_trm f xa = x) new_group = Set.filter (\<lambda>xa. meval_trm f xa = x) old_group" by auto
   assume assm: "(x, y) \<in>  group_multiset k b f X"
-  then have x_old_eval: "x \<in> meval_trm f ` old_group" by(auto simp: Let_def)
-  have "y = ecard (Set.filter (\<lambda>xa. meval_trm f xa = x) old_group)" using assm by(auto simp: Let_def)
+  then have x_old_eval: "x \<in> meval_trm f ` old_group" by auto
+  have "y = ecard (Set.filter (\<lambda>xa. meval_trm f xa = x) old_group)" using assm by auto
   then have "y =  ecard (Set.filter (\<lambda>xa. meval_trm f xa = x) new_group)" using aux1 diff_group by auto
-  then show "(x, y) \<in> group_multiset k b f (insert elem X)" using x_old_eval by (auto simp: Let_def)
+  then show "(x, y) \<in> group_multiset k b f (Set.insert elem X)" using x_old_eval by auto
 qed
 
 lemma multiset_new_term_insert:
   assumes elem_group: "drop b elem = k"
   and new_term_eval: "Set.filter (\<lambda>x. meval_trm f x = meval_trm f elem) (group k b X) = {}"
-  shows "group_multiset k b f (insert elem X) = insert (meval_trm f elem, 1) (group_multiset k b f X)"
+  shows "group_multiset k b f (Set.insert elem X) = Set.insert (meval_trm f elem, 1) (group_multiset k b f X)"
 proof -
   define updated_data where [simp]: "updated_data = X \<union> {elem}"
   define old_group where [simp]: "old_group = group k b X"
   define new_group where [simp]: "new_group = group k b updated_data"
   define old_evals where "old_evals = meval_trm f ` old_group"
-  have aux: "Set.filter (\<lambda>x. drop b x = k) (insert elem X) = insert elem old_group" using elem_group by auto
+  have aux: "Set.filter (\<lambda>x. drop b x = k) (Set.insert elem X) = Set.insert elem old_group" using elem_group by auto
   have aux1: "\<And>x. x \<noteq> meval_trm f elem \<Longrightarrow> Set.filter (\<lambda>xa. meval_trm f xa = x) new_group = Set.filter (\<lambda>xa. meval_trm f xa = x) old_group" by auto
   have aux2: "meval_trm f elem \<notin> old_evals" using new_term_eval by (auto simp: old_evals_def)
   moreover have "Set.filter (\<lambda>x. meval_trm f x = meval_trm f elem) new_group = {elem}" using new_term_eval elem_group by auto
@@ -420,8 +579,250 @@ proof -
   moreover have "(\<lambda>x. (x, ecard (Set.filter (\<lambda>xa. meval_trm f xa = x) new_group))) ` old_evals = 
                  (\<lambda>x. (x, ecard (Set.filter (\<lambda>xa. meval_trm f xa = x) old_group))) ` old_evals"
     using other_evals_unchanged by (metis (mono_tags, lifting) aux1 aux2 image_cong)
-  ultimately show "group_multiset k b f (insert elem X) = insert (meval_trm f elem, 1) (group_multiset k b f X)" using aux
-    by(simp add:Let_def old_evals_def)
+  ultimately show "group_multiset k b f (Set.insert elem X) = Set.insert (meval_trm f elem, 1) (group_multiset k b f X)" using aux
+    by(simp add: old_evals_def)
+qed
+
+lemma single_term_in_multiset:
+  assumes elem_group: "drop b elem = k"
+  and single_term_eval: "Set.filter (\<lambda>x. meval_trm f x = meval_trm f elem) (group k b X) = {elem}"
+  shows "(meval_trm f elem, 1) \<in> group_multiset k b f X"
+proof -
+  have "elem \<in> group k b X" using single_term_eval elem_group by(simp add:Set.filter_def) blast
+  then obtain v' where v'_def: "(meval_trm f elem, v') \<in> group_multiset k b f X" by auto fastforce
+  then have "v' = ecard (Set.filter (\<lambda>x. meval_trm f x = meval_trm f elem) (group k b X))" by auto
+  then have v'_val: "v' = 1" using single_term_eval by(simp add: ecard_def one_enat_def) 
+  then show "(meval_trm f elem, 1) \<in> group_multiset k b f X" using v'_def by auto
+qed
+
+lemma multiset_single_term_remove:
+  assumes elem_group: "drop b elem = k"
+  and single_term_eval: "Set.filter (\<lambda>x. meval_trm f x = meval_trm f elem) (group k b X) = {elem}"
+  shows "group_multiset k b f (X - {elem}) = (group_multiset k b f X) - {(meval_trm f elem, 1)}"
+proof (rule set_eqI, rule iffI)
+  fix x
+  assume x_in_M: "x \<in> group_multiset k b f (X - {elem})"
+  then obtain t v where x_def: "x = (t, v)" by fastforce
+  have "t \<in> meval_trm f ` group k b (X - {elem})" using x_def x_in_M by auto
+  moreover have "elem \<notin> group k b (X - {elem})" by auto
+  ultimately have noteq: "t \<noteq> meval_trm f elem" using imageE single_term_eval by auto
+  then have "x \<noteq> (meval_trm f elem, 1)" using x_def by force
+  moreover have "x \<in> group_multiset k b f X"
+    using  x_def by (metis Set.remove_def elem_group insert_Diff_single noteq other_evals_unchanged x_in_M)
+  ultimately show "x \<in>  (group_multiset k b f X) - {(meval_trm f elem, 1)}" 
+    by auto
+next
+  fix x
+  assume x_in_oldM: "x \<in> (group_multiset k b f X) - {(meval_trm f elem, 1)}"
+  then obtain t v where x_def: "x = (t, v)" by (meson surj_pair)
+  have "elem \<in> group k b X" using single_term_eval elem_group by(simp add:Set.filter_def) blast
+  have "(meval_trm f elem, 1) \<in> group_multiset k b f X" using single_term_in_multiset elem_group single_term_eval by auto
+  then have "t \<noteq> meval_trm f elem" using  x_def x_in_oldM by (metis DiffE insertI1 unique_term_multiset)
+  then show "x \<in> group_multiset k b f (X - {elem})" using x_def 
+    by (metis Set.member_remove Set.remove_def elem_group insert_Diff_single other_evals_unchanged x_in_oldM)
+qed
+
+lemma multiset_multiple_term_remove:
+  assumes elem_group: "drop b elem = k"
+  and old_term_eval: "Set.filter (\<lambda>x. meval_trm f x = meval_trm f elem) (group k b X) \<noteq> {elem}"
+  and old_val: "(meval_trm f elem, y) \<in> group_multiset k b f X" 
+  and inside: "elem \<in> X"
+  and finite: "finite X"
+  shows "group_multiset k b f (X - {elem}) = 
+         Set.insert (meval_trm f elem, y - 1) ((group_multiset k b f X) - {(meval_trm f elem, y)})"
+proof (rule set_eqI, rule iffI)
+  fix x
+  assume x_in_M: "x \<in> group_multiset k b f (X - {elem})"
+  then obtain t v where x_def: "x = (t, v)" by fastforce
+  define updated_data where "updated_data = X - {elem}"
+  define old_group where "old_group = group k b X"
+  define new_group where "new_group = group k b updated_data"
+  define old_evals where "old_evals = meval_trm f ` old_group"
+  have "Set.filter (\<lambda>x. meval_trm f x = meval_trm f elem) (group k b X) \<noteq> {}" using inside elem_group by auto
+  then obtain elem' where elem'_def:  "elem' \<in> Set.filter (\<lambda>x. meval_trm f x = meval_trm f elem) (group k b X) \<and> elem \<noteq> elem'" 
+    using old_term_eval by blast
+  have group_ins: "new_group = old_group - {elem}" using elem_group by (auto simp: new_group_def old_group_def updated_data_def)
+  have y_card: "y = ecard (Set.filter (\<lambda>xa. meval_trm f xa = meval_trm f elem) old_group)" using old_val by (auto simp: old_group_def)
+  have "Set.filter (\<lambda>xa. meval_trm f xa = meval_trm f elem) new_group = (Set.filter (\<lambda>xa. meval_trm f xa = meval_trm f elem) old_group) - {elem}"
+    using group_ins by fastforce
+  then have correct_card: "y - 1 = ecard (Set.filter (\<lambda>xa. meval_trm f xa = meval_trm f elem) new_group)" 
+    using y_card by (simp add: ecard_def elem_group enat_defs(2) inside old_group_def)
+  obtain v' where v'_def: "(meval_trm f elem, v') \<in> group_multiset k b f updated_data" using elem'_def 
+    by(simp add: updated_data_def) (metis (mono_tags) Set.member_filter imageI insert_Diff_single insert_iff)
+  then have "v' = y - 1" using correct_card by (auto simp: new_group_def)
+  then have aux1: "(meval_trm f elem, y - 1) \<in> group_multiset k b f updated_data" using v'_def by auto
+  have "y \<noteq> y - 1" using y_card by (smt (z3) Diff_insert_absorb Optimized_Agg.group_def cancel_comm_monoid_add_class.diff_cancel card.insert card_Diff_singleton_if diff_add_inverse2 ecard_def elem'_def enat.inject enat_defs(2) finite_Diff finite_filter idiff_enat_enat local.finite mk_disjoint_insert old_group_def plus_1_eq_Suc zero_neq_one)
+  then have aux2: "(meval_trm f elem, y) \<notin> group_multiset k b f (updated_data)" 
+    using unique_term_multiset[of "meval_trm f elem" "y - 1" k b f updated_data y] y_card aux1 by auto
+  show "x \<in> Set.insert (meval_trm f elem, y - 1) ((group_multiset k b f X) - {(meval_trm f elem, y)})"
+  proof (cases "t = meval_trm f elem")
+    case True
+    then have "v = y - 1" using x_in_M x_def aux1 using unique_term_multiset updated_data_def by blast
+    then show ?thesis using x_def x_in_M True by auto
+  next
+    case False
+    then show ?thesis using other_evals_unchanged by (metis Diff_iff elem_group insertI2 insert_Diff inside old.prod.inject singletonD x_def x_in_M)
+  qed
+next
+  fix x
+  assume x_in_oldM: "x \<in> Set.insert (meval_trm f elem, y - 1) ((group_multiset k b f X) - {(meval_trm f elem, y)})"
+  then obtain t v where x_def: "x = (t, v)" by force
+  define updated_data where "updated_data = X - {elem}"
+  define old_group where "old_group = group k b X"
+  define new_group where "new_group = group k b updated_data"
+  define old_evals where "old_evals = meval_trm f ` old_group"
+  have "Set.filter (\<lambda>x. meval_trm f x = meval_trm f elem) (group k b X) \<noteq> {}" using inside elem_group by auto
+  then obtain elem' where elem'_def:  "elem' \<in> Set.filter (\<lambda>x. meval_trm f x = meval_trm f elem) (group k b X) \<and> elem \<noteq> elem'" 
+    using old_term_eval by blast
+  have group_ins: "new_group = old_group - {elem}" using elem_group by (auto simp: new_group_def old_group_def updated_data_def)
+  have y_card: "y = ecard (Set.filter (\<lambda>xa. meval_trm f xa = meval_trm f elem) old_group)" using old_val by (auto simp: old_group_def)
+  have "Set.filter (\<lambda>xa. meval_trm f xa = meval_trm f elem) new_group = (Set.filter (\<lambda>xa. meval_trm f xa = meval_trm f elem) old_group) - {elem}"
+    using group_ins by fastforce
+  then have correct_card: "y - 1 = ecard (Set.filter (\<lambda>xa. meval_trm f xa = meval_trm f elem) new_group)" 
+    using y_card by (simp add: ecard_def elem_group enat_defs(2) inside old_group_def)
+  obtain v' where v'_def: "(meval_trm f elem, v') \<in> group_multiset k b f updated_data" using elem'_def 
+    by(simp add: updated_data_def) (metis (mono_tags) Set.member_filter imageI insert_Diff_single insert_iff)
+  then have "v' = y - 1" using correct_card by (auto simp: new_group_def)
+  then have aux1: "(meval_trm f elem, y - 1) \<in> group_multiset k b f updated_data" using v'_def by auto
+  show "x \<in> group_multiset k b f (X - {elem})" 
+  proof (cases "t = meval_trm f elem")
+    case True
+    then have "v = y - 1" using x_in_oldM x_def by (metis DiffE insertE old.prod.inject old_val singleton_iff unique_term_multiset)
+    then show ?thesis using True aux1 x_def updated_data_def by fastforce
+  next
+    case False
+    then show ?thesis by (metis DiffD1 elem_group insertE insert_Diff inside old.prod.inject other_evals_unchanged x_def x_in_oldM)
+  qed
+qed
+
+
+lemma multiset_old_term_insert:
+  assumes elem_group: "drop b elem = k"
+  and old_term_eval: "Set.filter (\<lambda>x. meval_trm f x = meval_trm f elem) (group k b X) \<noteq> {}"
+  and old_val: "(meval_trm f elem, y) \<in> group_multiset k b f X" 
+  and disjoint: "elem \<notin> X"
+  and finite: "finite X"
+  shows "group_multiset k b f (Set.insert elem X) = 
+         Set.insert (meval_trm f elem, y + 1) ((group_multiset k b f X) - {(meval_trm f elem, y)})"
+proof (rule set_eqI, rule iffI)
+  fix x
+  assume x_in_M: "x \<in> group_multiset k b f (Set.insert elem X)"
+  then obtain t v where x_def: "x = (t, v)" by fastforce
+  define updated_data where [simp]: "updated_data = X \<union> {elem}"
+  define old_group where [simp]: "old_group = group k b X"
+  define new_group where [simp]: "new_group = group k b updated_data"
+  define old_evals where "old_evals = meval_trm f ` old_group"
+  have group_ins: "new_group = Set.insert elem old_group" using elem_group by auto
+  have y_card: "y = ecard (Set.filter (\<lambda>xa. meval_trm f xa = meval_trm f elem) old_group)" using old_val by auto
+  moreover have "Set.filter (\<lambda>xa. meval_trm f xa = meval_trm f elem) (Set.insert elem (Set.filter (\<lambda>x. drop b x = k) X)) =
+                 Set.insert elem  (Set.filter (\<lambda>xa. meval_trm f xa = meval_trm f elem) (Set.filter (\<lambda>x. drop b x = k) X))" by auto
+  moreover have "elem \<notin> Set.filter (\<lambda>xa. meval_trm f xa = meval_trm f elem) (Set.filter (\<lambda>x. drop b x = k) X)" by (meson Set.member_filter disjoint)
+  ultimately have correct_card: "y + 1 = ecard (Set.filter (\<lambda>xa. meval_trm f xa = meval_trm f elem) new_group)" 
+    using eSuc_enat plus_1_eSuc(2) group_ins by(auto simp: ecard_def) 
+  then have aux1: "(meval_trm f elem, y + 1) \<in> group_multiset k b f (Set.insert elem X)" using group_ins by auto
+  have aux2: "(meval_trm f elem, y) \<notin> group_multiset k b f (Set.insert elem X)" 
+    using unique_term_multiset[of "meval_trm f elem" "y + 1" k b f updated_data y] aux1 y_card
+    by simp (meson ecard_def finite_filter finite valid_maggaux.simps)
+  show "x \<in> Set.insert (meval_trm f elem, y + 1) ((group_multiset k b f X) - {(meval_trm f elem, y)})"
+  proof (cases "t = meval_trm f elem")
+    case True
+    then have "v = y + 1" using x_in_M x_def aux1 using unique_term_multiset by blast
+    then show ?thesis using x_def x_in_M True by auto
+  next
+    case False
+    then show ?thesis using other_evals_unchanged 
+      by (metis DiffI elem_group insertI2 old.prod.inject singleton_iff x_def x_in_M)
+  qed
+next
+  fix x
+  assume x_in_oldM: "x \<in> Set.insert (meval_trm f elem, y + 1) ((group_multiset k b f X) - {(meval_trm f elem, y)})"
+  then obtain t v where x_def: "x = (t, v)" by force
+  define updated_data where [simp]: "updated_data = X \<union> {elem}"
+  define old_group where [simp]: "old_group = group k b X"
+  define new_group where [simp]: "new_group = group k b updated_data"
+  define old_evals where "old_evals = meval_trm f ` old_group"
+  have group_ins: "new_group = Set.insert elem old_group" using elem_group by auto
+  have y_card: "y = ecard (Set.filter (\<lambda>xa. meval_trm f xa = meval_trm f elem) old_group)" using old_val by auto
+  moreover have "Set.filter (\<lambda>xa. meval_trm f xa = meval_trm f elem) (Set.insert elem (Set.filter (\<lambda>x. drop b x = k) X)) =
+                 Set.insert elem  (Set.filter (\<lambda>xa. meval_trm f xa = meval_trm f elem) (Set.filter (\<lambda>x. drop b x = k) X))" by auto
+  moreover have "elem \<notin> Set.filter (\<lambda>xa. meval_trm f xa = meval_trm f elem) (Set.filter (\<lambda>x. drop b x = k) X)" by (meson Set.member_filter disjoint)
+  ultimately have correct_card: "y + 1 = ecard (Set.filter (\<lambda>xa. meval_trm f xa = meval_trm f elem) new_group)" 
+    using eSuc_enat plus_1_eSuc(2) group_ins by(auto simp: ecard_def) 
+  then have aux1: "(meval_trm f elem, y + 1) \<in> group_multiset k b f (Set.insert elem X)" using group_ins by auto
+  show "x \<in> group_multiset k b f (Set.insert elem X)" 
+  proof (cases "t = meval_trm f elem")
+    case True
+    then have "v = y + 1" using x_in_oldM x_def by (metis DiffE insertE old.prod.inject old_val singleton_iff unique_term_multiset)
+    then show ?thesis using True aux1 x_def by blast
+  next
+    case False
+    then show ?thesis by (metis DiffD1 elem_group insertE old.prod.inject other_evals_unchanged x_def x_in_oldM)
+  qed
+qed
+
+lemma length_flatten_multiset: 
+  assumes "finite M"
+  shows "length (flatten_multiset M) = Finite_Set.fold (\<lambda> (t, m) y. y + (the_enat m)) 0 M"
+  using length_fold[of "flatten_multiset M"] fold_flatten_multiset[of M "(\<lambda>_ n. n + 1)" 0]
+  by (simp add: fold_flatten_multiset assms comp_fun_commute.intro) (meson add.commute)
+
+lemma length_flatten_multiset':
+  assumes "finite X"
+  shows "length (flatten_multiset(group_multiset k b f X)) = card (group k b X)"
+  using assms
+proof(induction X)
+  case empty
+  then have "group k b {} = {}" by auto
+  then show ?case using length_flatten_multiset by auto
+next
+  case (insert elem F)
+  define updated_data where [simp]: "updated_data = Set.insert elem F"
+  define group where [simp]: "group = Set.filter (\<lambda>x. drop b x = k) updated_data"
+  define M where [simp]: "M = (\<lambda>y. (y, ecard (Set.filter (\<lambda>x. meval_trm f x = y) group))) ` meval_trm f ` group"
+  define old_group where [simp]: "old_group = Set.filter (\<lambda>x. drop b x = k) F"
+  define old_M where [simp]: "old_M = (\<lambda>y. (y, ecard (Set.filter (\<lambda>x. meval_trm f x = y) old_group))) ` meval_trm f ` old_group"
+  define old_evals where "old_evals = meval_trm f ` old_group"
+  interpret comp_fun_commute "\<lambda>(t, m) y. y + the_enat m" by unfold_locales auto
+  have both_finite: "finite M \<and> finite old_M" using insert by auto
+  show ?case
+  proof(cases "drop b elem = k")
+    case True
+    then have group_elem: "drop b elem = k" by auto
+    have "length(flatten_multiset(M)) = length(flatten_multiset(old_M)) + 1" 
+    proof(cases "Set.filter (\<lambda>x. meval_trm f x = meval_trm f elem) old_group = {}")
+      case True
+      then have "M = Set.insert (meval_trm f elem, 1) old_M" using multiset_new_term_insert True group_elem by simp
+      moreover have "(meval_trm f elem, 1) \<notin> old_M" using True by auto
+      ultimately show ?thesis using both_finite length_flatten_multiset by (simp add: enat_defs(2) length_flatten_multiset)
+    next
+      case False
+      then obtain y where y_def: "(meval_trm f elem, y) \<in> old_M" 
+        by (smt (z3) Collect_empty_eq Set.filter_def image_eqI old_M_def)
+      then obtain xa where xa_def: "y = ecard (Set.filter (\<lambda>x. meval_trm f x = meval_trm f xa) (Set.filter (\<lambda>x. drop b x = drop b xa) F))" 
+        by(auto)
+      have aux1: "finite (Set.filter (\<lambda>x. meval_trm f x = meval_trm f xa) (Set.filter (\<lambda>x. drop b x = drop b xa) F))" using insert by auto
+      then obtain i where i_def: "y = i" by auto
+      have finite_remove: "finite (old_M - {(meval_trm f elem, y)})" using both_finite finite_Diff  by (auto simp: Set.remove_def)
+      have finite_insert: "finite (Set.insert (meval_trm f elem, y) old_M)" using both_finite by blast
+      have M_insert_remove_def: "M = Set.insert (meval_trm f elem, y + 1) (old_M - {(meval_trm f elem, y)})" 
+        using multiset_old_term_insert group_elem False y_def insert
+        by(simp only: M_def old_M_def group_def old_group_def updated_data_def group_multiset_def Let_def Optimized_Agg.group_def) auto
+      then have aux: "length(flatten_multiset(Set.insert (meval_trm f elem, y) old_M)) = length(flatten_multiset(old_M - {(meval_trm f elem, y)})) + i" 
+        using both_finite finite_insert finite_remove Finite_Set.comp_fun_commute.fold_insert_remove[of "\<lambda>(t, m) y. y + the_enat m" old_M 0 "(meval_trm f elem, y)"]
+        by (simp only: length_flatten_multiset) (metis aux1 comp_fun_commute_axioms ecard_def i_def old.prod.case plus_enat_simps(1) the_enat.simps xa_def)
+      have "(meval_trm f elem, y + 1) \<notin> old_M - {(meval_trm f elem, y)}" using y_def by auto
+      then show ?thesis using both_finite finite_remove M_insert_remove_def i_def Finite_Set.comp_fun_commute.fold_insert[of "\<lambda>(t, m) y. y + the_enat m" "old_M - {(meval_trm f elem, y)}" "(meval_trm f elem, y + 1)" 0]
+        by (smt (z3) add.commute add.left_commute aux1 case_prod_conv comp_fun_commute_axioms ecard_def fold_insert_remove insert_absorb length_flatten_multiset one_enat_def plus_enat_simps(1) the_enat.simps xa_def y_def)
+    qed
+    moreover have "group = Set.insert elem old_group"
+      using True insert by(auto) 
+    ultimately show ?thesis using insert by auto
+  next
+    case False
+    then have aux: "Optimized_Agg.group k b (Set.insert elem F) = Optimized_Agg.group k b F" by auto
+    then have "group_multiset k b f (Set.insert elem F) = group_multiset k b f F" by auto
+    then show ?thesis using aux insert by auto
+  qed
 qed
 
 lemma foldl_eint_equival: 
@@ -435,70 +836,6 @@ case Nil
 next
   case (Cons a X)
   then show ?case using Cons by auto
-qed
-
-lemma multiset_old_term_insert:
-  assumes elem_group: "drop b elem = k"
-  and old_term_eval: "Set.filter (\<lambda>x. meval_trm f x = meval_trm f elem) (group k b X) \<noteq> {}"
-  and old_val: "(meval_trm f elem, y) \<in> group_multiset k b f X" 
-  and disjoint: "elem \<notin> X"
-  and finite: "finite X"
-  shows "group_multiset k b f (insert elem X) = 
-         insert (meval_trm f elem, y + 1) ((group_multiset k b f X) - {(meval_trm f elem, y)})"
-proof (rule set_eqI, rule iffI)
-  fix x
-  assume x_in_M: "x \<in> group_multiset k b f (insert elem X)"
-  then obtain t v where x_def: "x = (t, v)" by fastforce
-  define updated_data where [simp]: "updated_data = X \<union> {elem}"
-  define old_group where [simp]: "old_group = group k b X"
-  define new_group where [simp]: "new_group = group k b updated_data"
-  define old_evals where "old_evals = meval_trm f ` old_group"
-  have group_ins: "new_group = insert elem old_group" using elem_group by auto
-  have y_card: "y = ecard (Set.filter (\<lambda>xa. meval_trm f xa = meval_trm f elem) old_group)" using old_val by (auto simp: Let_def)
-  moreover have "Set.filter (\<lambda>xa. meval_trm f xa = meval_trm f elem) (insert elem (Set.filter (\<lambda>x. drop b x = k) X)) =
-                 insert elem  (Set.filter (\<lambda>xa. meval_trm f xa = meval_trm f elem) (Set.filter (\<lambda>x. drop b x = k) X))" by auto
-  moreover have "elem \<notin> Set.filter (\<lambda>xa. meval_trm f xa = meval_trm f elem) (Set.filter (\<lambda>x. drop b x = k) X)" by (meson Set.member_filter disjoint)
-  ultimately have correct_card: "y + 1 = ecard (Set.filter (\<lambda>xa. meval_trm f xa = meval_trm f elem) new_group)" 
-    using eSuc_enat plus_1_eSuc(2) group_ins by(auto simp: ecard_def) 
-  then have aux1: "(meval_trm f elem, y + 1) \<in> group_multiset k b f (insert elem X)" using group_ins by (auto simp:Let_def)
-  have aux2: "(meval_trm f elem, y) \<notin> group_multiset k b f (insert elem X)" 
-    using unique_term_multiset[of "meval_trm f elem" "y + 1" k b f updated_data y] aux1 y_card
-    by(simp add:Let_def) (meson ecard_def finite_filter finite valid_maggaux.simps)
-  show "x \<in> insert (meval_trm f elem, y + 1) ((group_multiset k b f X) - {(meval_trm f elem, y)})"
-  proof (cases "t = meval_trm f elem")
-    case True
-    then have "v = y + 1" using x_in_M x_def aux1 using unique_term_multiset by blast
-    then show ?thesis using x_def x_in_M True by auto
-  next
-    case False
-    then show ?thesis using other_evals_unchanged 
-      by (metis DiffI elem_group insertI2 old.prod.inject singleton_iff x_def x_in_M)
-  qed
-next
-  fix x
-  assume x_in_oldM: "x \<in> insert (meval_trm f elem, y + 1) ((group_multiset k b f X) - {(meval_trm f elem, y)})"
-  then obtain t v where x_def: "x = (t, v)" by force
-  define updated_data where [simp]: "updated_data = X \<union> {elem}"
-  define old_group where [simp]: "old_group = group k b X"
-  define new_group where [simp]: "new_group = group k b updated_data"
-  define old_evals where "old_evals = meval_trm f ` old_group"
-  have group_ins: "new_group = insert elem old_group" using elem_group by auto
-  have y_card: "y = ecard (Set.filter (\<lambda>xa. meval_trm f xa = meval_trm f elem) old_group)" using old_val by (auto simp: Let_def)
-  moreover have "Set.filter (\<lambda>xa. meval_trm f xa = meval_trm f elem) (insert elem (Set.filter (\<lambda>x. drop b x = k) X)) =
-                 insert elem  (Set.filter (\<lambda>xa. meval_trm f xa = meval_trm f elem) (Set.filter (\<lambda>x. drop b x = k) X))" by auto
-  moreover have "elem \<notin> Set.filter (\<lambda>xa. meval_trm f xa = meval_trm f elem) (Set.filter (\<lambda>x. drop b x = k) X)" by (meson Set.member_filter disjoint)
-  ultimately have correct_card: "y + 1 = ecard (Set.filter (\<lambda>xa. meval_trm f xa = meval_trm f elem) new_group)" 
-    using eSuc_enat plus_1_eSuc(2) group_ins by(auto simp: ecard_def) 
-  then have aux1: "(meval_trm f elem, y + 1) \<in> group_multiset k b f (insert elem X)" using group_ins by (auto simp:Let_def)
-  show "x \<in> group_multiset k b f (insert elem X)" 
-  proof (cases "t = meval_trm f elem")
-    case True
-    then have "v = y + 1" using x_in_oldM x_def by (metis DiffE insertE old.prod.inject old_val singleton_iff unique_term_multiset)
-    then show ?thesis using True aux1 x_def by blast
-  next
-    case False
-    then show ?thesis by (metis DiffD1 elem_group insertE old.prod.inject other_evals_unchanged x_def x_in_oldM)
-  qed
 qed
 
 lemma finite_set_fold_int:
@@ -539,13 +876,13 @@ proof -
     assume assm: "k \<in> (drop b) ` updated_data"
     show "k \<in>  Mapping.keys updated_map"
       using valid_before assm
-      by (cases "k \<in> (drop b) ` X") (auto simp: Let_def split:option.splits)
+      by (cases "k \<in> (drop b) ` X") (auto split:option.splits)
   next
     fix k
     assume assm: "k \<in> Mapping.keys updated_map"
     show "k \<in> (drop b) ` updated_data"
       using valid_before assm
-      by (cases "k \<in> Mapping.keys m") (auto simp: Let_def split:option.splits)
+      by (cases "k \<in> Mapping.keys m") (auto split:option.splits)
   qed
   have valid_value_invariant: "\<And>k. k \<in> Mapping.keys updated_map \<longrightarrow> Mapping.lookup updated_map k = 
           (let group = Set.filter (\<lambda>x. drop b x = k) updated_data;
@@ -565,10 +902,10 @@ proof -
     define term' where [simp]: "term' = meval_trm f elem"
     assume assm: "k \<in> Mapping.keys updated_map"
     have finite: "finite M" using valid_before by auto
-    have y0_int: "y0 \<in> range EInt" using type_restr valid_before by (auto simp:Let_def type_restr_def)
-    have multiset_int: "\<And>t m. (t, m) \<in> M \<Longrightarrow> t \<in> range EInt" using type_restr valid_before by (auto simp: type_restr_def Let_def image_subset_iff)  
+    have y0_int: "y0 \<in> range EInt" using type_restr valid_before by (auto simp: type_restr_def)
+    have multiset_int: "\<And>t m. (t, m) \<in> M \<Longrightarrow> t \<in> range EInt" using type_restr valid_before by (auto simp: type_restr_def image_subset_iff)  
     then have M_int: "set (flatten_multiset M) \<subseteq> range EInt" using flatten_multiset_eint[of M] finite by auto
-    have old_multiset_int: "\<And>t m. (t, m) \<in> old_M \<Longrightarrow> t \<in> range EInt" using type_restr valid_before by (auto simp: type_restr_def Let_def image_subset_iff)  
+    have old_multiset_int: "\<And>t m. (t, m) \<in> old_M \<Longrightarrow> t \<in> range EInt" using type_restr valid_before by (auto simp: type_restr_def image_subset_iff)  
     then have M_old_int: "set (flatten_multiset old_M) \<subseteq> range EInt" using flatten_multiset_eint[of old_M] finite valid_before by auto
     show "Mapping.lookup updated_map k = 
           (let group = Set.filter (\<lambda>x. drop b x = k) updated_data;
@@ -580,14 +917,14 @@ proof -
     proof (cases "k \<in> Mapping.keys m")
       case False
       then have map_val: "Mapping.lookup updated_map k = Some (1, y0 + term')" 
-        using assm valid_before by (auto simp: keys_is_none_rep Let_def lookup_update' split:option.splits)
+        using assm valid_before by (auto simp: keys_is_none_rep lookup_update' split:option.splits)
       have "drop b elem = k" 
         using assm False 
-        by(auto simp: Let_def split:option.splits)
+        by(auto simp: split:option.splits)
       then have group_single_elem: "group = {elem}" 
         using False valid_before image_iff
-        by(auto) (metis False imageI)
-      then have M_single: "M = insert (meval_trm f elem, enat 1) {}"
+        by auto fastforce+
+      then have M_single: "M = Set.insert (meval_trm f elem, enat 1) {}"
         using group_single_elem unfolding M_def Set.filter_def ecard_def by (auto cong: conj_cong)
       then have correct_len: "length(flatten_multiset(M)) = 1" 
         using length_flatten_multiset[of M] Finite_Set.comp_fun_commute.fold_insert by simp
@@ -595,7 +932,7 @@ proof -
         using foldl_eint_equival y0_int M_int by auto
       moreover have "foldl (plus') y0 (flatten_multiset M) = Finite_Set.fold (\<lambda>(t, m). (plus') t ^^ the_enat m) y0 M"
         using foldl_flatten_multiset[of M plus' y0] comp_fun_commute_plus' comm_plus'  finite by auto
-      moreover have "Finite_Set.fold (\<lambda>(t, m). plus' t ^^ the_enat m) y0 (insert (meval_trm f elem, enat 1) {}) = plus' y0 term'"
+      moreover have "Finite_Set.fold (\<lambda>(t, m). plus' t ^^ the_enat m) y0 (Set.insert (meval_trm f elem, enat 1) {}) = plus' y0 term'"
         using  Finite_Set.comp_fun_commute.fold_insert[of "\<lambda>(t, m). plus' t ^^ the_enat m"] finite plus'_comp_commute comm_plus' by auto
       moreover have "meval_trm f elem \<in> range EInt" using valid_before multiset_int M_single by blast
       ultimately have "foldl plus y0 (flatten_multiset(M)) = y0 + term'" using M_single y0_int by force
@@ -607,18 +944,18 @@ proof -
       proof(cases "drop b elem = k")
         case True
         then have elem_group: "drop b elem = k" by auto
-        then have newgroup_def: "group = insert elem old_group" by auto
+        then have newgroup_def: "group = Set.insert elem old_group" by auto
         have both_finite: "finite old_M \<and> finite M" using valid_before by auto
         obtain len sum where lookup_val: "Mapping.lookup m k = Some(len, sum)" 
           by (metis domIff in_map keys_dom_lookup not_Some_eq prod.exhaust_sel)
-        have len_def: "len = length(flatten_multiset(old_M))" using lookup_val in_map valid_before by(auto simp:Let_def)
-        moreover have sum_def: "sum = foldl plus y0 (flatten_multiset old_M)" using lookup_val in_map valid_before by(auto simp:Let_def)
+        have len_def: "len = length(flatten_multiset(old_M))" using lookup_val in_map valid_before by auto
+        moreover have sum_def: "sum = foldl plus y0 (flatten_multiset old_M)" using lookup_val in_map valid_before by auto
         ultimately have "Mapping.lookup updated_map k = Some (len + 1, sum + term')"
-          using lookup_val True by(simp add: lookup_update Let_def)
+          using lookup_val True by(simp add: lookup_update)
         moreover have "length(flatten_multiset(M)) = length(flatten_multiset(old_M)) + 1"
         proof(cases "Set.filter (\<lambda>x. meval_trm f x = meval_trm f elem) old_group = {}")
           case True
-          then have "M = insert (meval_trm f elem, 1) old_M" using multiset_new_term_insert elem_group by(simp add: Let_def)
+          then have "M = Set.insert (meval_trm f elem, 1) old_M" using multiset_new_term_insert elem_group by simp
           moreover have "(meval_trm f elem, 1) \<notin> old_M" using True by auto
           ultimately show ?thesis using both_finite by (auto simp:length_flatten_multiset one_enat_def)
         next
@@ -628,11 +965,11 @@ proof -
           then obtain i where i_def: "y = enat i" 
             by (smt (z3) Pair_inject ecard_def finite_filter image_iff old_M_def old_group_def valid_before valid_maggaux.simps)
           have finite_remove: "finite (old_M - {(meval_trm f elem, y)})" using both_finite finite_Diff  by (auto simp: Set.remove_def)
-          have finite_insert: "finite (insert (meval_trm f elem, y) old_M)" using both_finite by blast
-          have M_insert_remove_def: "M = insert (meval_trm f elem, y + 1) (old_M - {(meval_trm f elem, y)})" 
+          have finite_insert: "finite (Set.insert (meval_trm f elem, y) old_M)" using both_finite by blast
+          have M_insert_remove_def: "M = Set.insert (meval_trm f elem, y + 1) (old_M - {(meval_trm f elem, y)})" 
             using multiset_old_term_insert[of b elem k f X y] elem_group False y_def valid_before disjoint
             by(simp only: M_def old_M_def group_def old_group_def updated_data_def group_multiset_def Let_def Optimized_Agg.group_def) auto          
-          then have aux: "length(flatten_multiset(insert (meval_trm f elem, y) old_M)) = length(flatten_multiset(old_M - {(meval_trm f elem, y)})) + i" 
+          then have aux: "length(flatten_multiset(Set.insert (meval_trm f elem, y) old_M)) = length(flatten_multiset(old_M - {(meval_trm f elem, y)})) + i" 
             using both_finite length_flatten_multiset finite_insert i_def len_commute
             Finite_Set.comp_fun_commute.fold_insert_remove[of "\<lambda>(t, m) y. y + the_enat m" old_M 0 "(meval_trm f elem, y)"] by auto
           have "(meval_trm f elem, y + 1) \<notin> old_M - {(meval_trm f elem, y)}" using y_def by auto
@@ -643,7 +980,7 @@ proof -
         moreover have "foldl plus y0 (flatten_multiset M) = (foldl plus y0 (flatten_multiset old_M)) + term'"
         proof(cases "Set.filter (\<lambda>x. meval_trm f x = meval_trm f elem) old_group = {}")
           case True
-          then have "M = insert (meval_trm f elem, 1) old_M" using multiset_new_term_insert elem_group by(simp add: Let_def)
+          then have "M = Set.insert (meval_trm f elem, 1) old_M" using multiset_new_term_insert elem_group by simp
           moreover have "(meval_trm f elem, 1) \<notin> old_M" using True by auto
           moreover have "foldl (+) y0 (flatten_multiset M) = Finite_Set.fold (\<lambda>(t, m). (plus') t ^^ the_enat m) y0 M"
             using foldl_flatten_multiset foldl_eint_equival M_int y0_int both_finite comm_plus' comp_fun_commute_plus' by(simp)
@@ -662,16 +999,16 @@ proof -
           then obtain i where i_def: "y = enat i" 
             by (smt (z3) Pair_inject ecard_def finite_filter image_iff old_M_def old_group_def valid_before valid_maggaux.simps)
           have finite_remove: "finite (old_M - {(meval_trm f elem, y)})" using both_finite finite_Diff  by (auto simp: Set.remove_def)
-          have finite_insert: "finite (insert (meval_trm f elem, y) old_M)" using both_finite by blast
-          have M_insert_remove_def: "M = insert (meval_trm f elem, y + 1) (old_M - {(meval_trm f elem, y)})" 
+          have finite_insert: "finite (Set.insert (meval_trm f elem, y) old_M)" using both_finite by blast
+          have M_insert_remove_def: "M = Set.insert (meval_trm f elem, y + 1) (old_M - {(meval_trm f elem, y)})" 
             using multiset_old_term_insert[of b elem k f X y] elem_group False y_def valid_before disjoint
             by(simp only: M_def old_M_def group_def old_group_def updated_data_def group_multiset_def Let_def Optimized_Agg.group_def) auto 
           have foldl_plus_plus'_equiv: "foldl (+) y0 (flatten_multiset M) = foldl (plus') y0 (flatten_multiset M)" using foldl_eint_equival M_int y0_int by auto
-          have aux1: "foldl (plus') y0 (flatten_multiset (insert (term', y) old_M)) = Finite_Set.fold (\<lambda>(t, m). (plus') t ^^ the_enat m) y0 (insert (term', y) old_M)"
-            using foldl_flatten_multiset[of "insert (term', y) old_M" plus' y0] finite_insert comp_fun_commute_plus' comm_plus' by auto
+          have aux1: "foldl (plus') y0 (flatten_multiset (Set.insert (term', y) old_M)) = Finite_Set.fold (\<lambda>(t, m). (plus') t ^^ the_enat m) y0 (Set.insert (term', y) old_M)"
+            using foldl_flatten_multiset[of "Set.insert (term', y) old_M" plus' y0] finite_insert comp_fun_commute_plus' comm_plus' by auto
           moreover have foldl_remove_equiv: "foldl plus' y0 (flatten_multiset(old_M - {(term', y)})) = Finite_Set.fold (\<lambda>(t, m). (plus') t ^^ the_enat m) y0 (old_M - {(term', y)})"
             using foldl_flatten_multiset[of "old_M - {(term', y)}" plus' y0] finite_insert comp_fun_commute_plus' comm_plus' by auto
-          ultimately have aux: "foldl plus' y0 (flatten_multiset(insert (term', y) old_M)) = ((plus' term') ^^ (the_enat y)) (foldl plus' y0 (flatten_multiset(old_M - {(term', y)})))" 
+          ultimately have aux: "foldl plus' y0 (flatten_multiset(Set.insert (term', y) old_M)) = ((plus' term') ^^ (the_enat y)) (foldl plus' y0 (flatten_multiset(old_M - {(term', y)})))" 
             using  finite_insert plus'_comp_commute Finite_Set.comp_fun_commute.fold_insert_remove[of "\<lambda>(t, m). (plus') t ^^ the_enat m"] by auto
           moreover have term'_int: "term' \<in> range EInt" using old_multiset_int term'_def y_def by blast
           moreover have "foldl plus' y0 (flatten_multiset(old_M - {(term', y)})) \<in> range EInt" 
@@ -685,7 +1022,7 @@ proof -
           moreover have "foldl (plus') y0 (flatten_multiset(M)) = Finite_Set.fold (\<lambda>(t, m). (plus') t ^^ the_enat m) y0 M"
             using foldl_flatten_multiset[of M plus' y0] both_finite comp_fun_commute_plus' comm_plus' by auto
           ultimately have "foldl (plus') y0 (flatten_multiset(M)) = plus' term' (foldl plus' y0 (flatten_multiset(old_M)))"
-            using aux1 by (smt (z3) add.commute aux both_finite comp_eq_dest_lhs comp_fun_commute.fold_insert_remove foldl_remove_equiv funpow_add i_def insert_absorb old.prod.case plus'_comp_commute plus'_iter_one term'_def the_enat.simps y_def)
+            using aux1 by (smt (z3) add.commute aux comp_eq_dest_lhs comp_fun_commute.fold_insert comp_fun_commute.fold_insert_remove finite_remove foldl_remove_equiv funpow_add i_def insert_Diff insert_Diff_single old.prod.case one_enat_def plus'_comp_commute plus'_iter_one_enat term'_def the_enat.simps y_def)
           moreover have "foldl plus' y0 (flatten_multiset(old_M)) \<in> range EInt" 
             by (metis aux1 both_finite finite_set_fold_int insert_absorb old_multiset_int term'_def y0_int y_def)
           ultimately show ?thesis 
@@ -697,16 +1034,16 @@ proof -
         then have same_group: "group = old_group" by auto
         then have "M = old_M" by auto
         then have "Mapping.lookup updated_map k = Mapping.lookup m k" 
-          using False by (auto split:option.splits simp:Let_def lookup_update')
+          using False by (auto split:option.splits simp: lookup_update')
         then show ?thesis using valid_before same_group in_map 
-          by (auto simp: Let_def)
+          by auto
       qed
     qed
   qed
-  have valid_type_restr: "type_restr \<lparr>aggargs_cols = cols, aggargs_n = n, aggargs_g0 = g0, aggargs_y = y, aggargs_\<omega> = \<omega>, aggargs_b = b, aggargs_f = f\<rparr> (insert elem X)"
-    using valid_before type_restr by (auto simp:type_restr_def Let_def)
+  have valid_type_restr: "type_restr \<lparr>aggargs_cols = cols, aggargs_n = n, aggargs_g0 = g0, aggargs_y = y, aggargs_\<omega> = \<omega>, aggargs_b = b, aggargs_f = f\<rparr> (Set.insert elem X)"
+    using valid_before type_restr by (auto simp:type_restr_def)
   show ?thesis using valid_value_invariant valid_key_invariant valid_finite valid_before valid_type_restr
-    by (auto simp:Let_def)
+    by auto
 qed
 
 lemma valid_insert_cnt_unfolded: 
@@ -726,13 +1063,13 @@ proof -
     assume assm: "k \<in> (drop b) ` updated_data"
     show "k \<in>  Mapping.keys updated_map"
       using valid_before assm
-      by (cases "k \<in> (drop b) ` X") (auto simp: Let_def split:option.splits)
+      by (cases "k \<in> (drop b) ` X") (auto split:option.splits)
   next
     fix k
     assume assm: "k \<in> Mapping.keys updated_map"
     show "k \<in> (drop b) ` updated_data"
       using valid_before assm
-      by (cases "k \<in> Mapping.keys m") (auto simp: Let_def split:option.splits)
+      by (cases "k \<in> Mapping.keys m") (auto split:option.splits)
   qed
   have valid_value_invariant: "\<And>k. k \<in> Mapping.keys updated_map \<longrightarrow> Mapping.lookup updated_map k = 
           (let group = Set.filter (\<lambda>x. drop b x = k) updated_data;
@@ -753,14 +1090,14 @@ proof -
     proof (cases "k \<in> Mapping.keys m")
       case False
       then have map_val: "Mapping.lookup updated_map k = Some 1" 
-        using assm by (auto simp: keys_is_none_rep Let_def lookup_update' split:option.splits)
+        using assm by (auto simp: keys_is_none_rep lookup_update' split:option.splits)
       have "drop b elem = k" 
         using assm False 
-        by(auto simp: Let_def split:option.splits)
+        by(auto  split:option.splits)
       then have group_single_elem: "group = {elem}" 
         using False valid_before image_iff
         by fastforce
-      then have "M = insert (meval_trm f elem, enat 1) {}"
+      then have "M = Set.insert (meval_trm f elem, enat 1) {}"
         using group_single_elem unfolding M_def Set.filter_def ecard_def by (auto cong: conj_cong)
       then have "length(flatten_multiset M) = 1" 
         using length_flatten_multiset[of M] Finite_Set.comp_fun_commute.fold_insert by(auto)
@@ -772,12 +1109,12 @@ proof -
       proof(cases "drop b elem = k")
         case True
         then have elem_group: "drop b elem = k" by auto
-        then have newgroup_def: "group = insert elem old_group" by auto
+        then have newgroup_def: "group = Set.insert elem old_group" by auto
         have both_finite: "finite old_M \<and> finite M" using valid_before by auto
         have "length(flatten_multiset(M)) = length(flatten_multiset(old_M)) + 1"
         proof(cases "Set.filter (\<lambda>x. meval_trm f x = meval_trm f elem) old_group = {}")
           case True
-          then have "M = insert (meval_trm f elem, 1) old_M" using multiset_new_term_insert elem_group by(simp add: Let_def)
+          then have "M = Set.insert (meval_trm f elem, 1) old_M" using multiset_new_term_insert elem_group by simp
           moreover have "(meval_trm f elem, 1) \<notin> old_M" using True by auto
           ultimately show ?thesis using both_finite by (auto simp:length_flatten_multiset one_enat_def)
         next
@@ -787,11 +1124,11 @@ proof -
           then obtain i where i_def: "y = enat i" 
             by (smt (z3) Pair_inject ecard_def finite_filter image_iff old_M_def old_group_def valid_before valid_maggaux.simps)
           have finite_remove: "finite (old_M - {(meval_trm f elem, y)})" using both_finite finite_Diff  by (auto simp: Set.remove_def)
-          have finite_insert: "finite (insert (meval_trm f elem, y) old_M)" using both_finite by blast
-          have M_insert_remove_def: "M = insert (meval_trm f elem, y + 1) (old_M - {(meval_trm f elem, y)})" 
+          have finite_insert: "finite (Set.insert (meval_trm f elem, y) old_M)" using both_finite by blast
+          have M_insert_remove_def: "M = Set.insert (meval_trm f elem, y + 1) (old_M - {(meval_trm f elem, y)})" 
             using multiset_old_term_insert[of b elem k f X y] elem_group False y_def valid_before disjoint
             by(simp only: M_def old_M_def group_def old_group_def updated_data_def group_multiset_def Let_def Optimized_Agg.group_def) auto          
-          then have aux: "length(flatten_multiset(insert (meval_trm f elem, y) old_M)) = length(flatten_multiset(old_M - {(meval_trm f elem, y)})) + i" 
+          then have aux: "length(flatten_multiset(Set.insert (meval_trm f elem, y) old_M)) = length(flatten_multiset(old_M - {(meval_trm f elem, y)})) + i" 
             using both_finite finite_insert finite_remove 
             Finite_Set.comp_fun_commute.fold_insert_remove[of "\<lambda>(t, m) y. y + the_enat m" old_M 0 "(meval_trm f elem, y)"]
             by (simp only: length_flatten_multiset) (metis comp_fun_commute_axioms i_def old.prod.case the_enat.simps)
@@ -800,7 +1137,7 @@ proof -
             by (metis (mono_tags, lifting) aux case_prod_conv comp_fun_commute_axioms group_cancel.add1 insert_absorb length_flatten_multiset one_enat_def plus_enat_simps(1) the_enat.simps y_def)
         qed
         moreover obtain len where len_def: "Mapping.lookup m k = Some len \<and> len = length(flatten_multiset(old_M))" 
-          using valid_before in_map by auto metis
+          using valid_before in_map by auto
         then have "Mapping.lookup updated_map k = Some (len + 1)" by (simp add: elem_group lookup_update)
         ultimately show ?thesis by (simp add: len_def)
       next
@@ -808,14 +1145,14 @@ proof -
         then have same_group: "group = old_group" by auto
         then have "M = old_M" by auto
         then have "Mapping.lookup updated_map k = Mapping.lookup m k" 
-          using False by (auto split:option.splits simp:Let_def lookup_update')
+          using False by (auto split:option.splits simp: lookup_update')
         then show ?thesis using valid_before same_group in_map 
-          by (auto simp: Let_def)
+          by auto
       qed
     qed
   qed
   show ?thesis using valid_value_invariant valid_key_invariant valid_finite valid_before
-    by (auto simp add: Let_def)
+    by auto
 qed
 
 lemma valid_insert_maggaux_unfolded: 
@@ -841,14 +1178,14 @@ proof(induction aux)
     obtain intermediate_map where intermediate_map_def: "CntAux intermediate_map = insert_maggaux args F (CntAux m)" by auto
     have valid_a: "valid_maggaux args (CntAux (insert_cnt args x intermediate_map)) (X \<union> F \<union> {x})" 
       using insert valid_insert_cnt_unfolded disjoint Un_iff args_def intermediate_map_def by (metis disjoint_insert(1))
-    then have "Finite_Set.fold (insert_cnt args) m (insert x F) = insert_cnt args x (Finite_Set.fold (insert_cnt args) m F)"
+    then have "Finite_Set.fold (insert_cnt args) m (Set.insert x F) = insert_cnt args x (Finite_Set.fold (insert_cnt args) m F)"
       using  Finite_Set.comp_fun_commute.fold_insert[of "insert_cnt args" F x m] insert by auto
     moreover have "CntAux (Finite_Set.fold (insert_cnt args) m F) = CntAux intermediate_map"
       by(auto simp:intermediate_map_def)
-    ultimately have "insert_maggaux args (insert x F) (CntAux m) = CntAux (insert_cnt args x intermediate_map)"
+    ultimately have "insert_maggaux args (Set.insert x F) (CntAux m) = CntAux (insert_cnt args x intermediate_map)"
       using  Finite_Set.comp_fun_commute.fold_insert[of "insert_cnt args" F x m]
       by auto
-    then have "valid_maggaux args (insert_maggaux args (insert x F) (CntAux m)) (X \<union> insert x F)"
+    then have "valid_maggaux args (insert_maggaux args (Set.insert x F) (CntAux m)) (X \<union> Set.insert x F)"
       using valid_a
       by auto
     then show ?case
@@ -872,65 +1209,426 @@ next
     obtain intermediate_map where intermediate_map_def: "SumAux intermediate_map = insert_maggaux args F (SumAux m)" by auto
     then have intermediate_map_def': "intermediate_map = Finite_Set.fold (insert_sum args) m F" by auto
     have "X \<inter> F = {}" using insert(4) by auto
-    moreover have "type_restr args F" using insert(5)  by (cases "fst \<omega>") (auto simp: args_def type_restr_def Let_def) 
+    moreover have "type_restr args F" using insert(5)  by (cases "fst \<omega>") (auto simp: args_def type_restr_def) 
     moreover have "valid_maggaux args (SumAux m) X" using valid_before by (auto simp:args_def)
     ultimately have valid_int: "valid_maggaux args (SumAux intermediate_map) (X \<union> F)" using insert(3) by(simp only:intermediate_map_def args_def)
     moreover have "x \<notin> X \<union> F" using insert(2) insert.prems(1) by auto
-    moreover have type_x: "type_restr args {x}" using insert(5) by (cases "fst \<omega>") (auto simp: args_def type_restr_def Let_def) 
+    moreover have type_x: "type_restr args {x}" using insert(5) by (cases "fst \<omega>") (auto simp: args_def type_restr_def) 
     ultimately have valid_a: "valid_maggaux args (SumAux (insert_sum args x intermediate_map)) (X \<union> F \<union> {x})" 
       using valid_insert_sum_unfolded[of cols n g0 y \<omega> b f intermediate_map "(X \<union> F)" x] by(auto simp: args_def)
-    have y0_int: "snd (aggargs_\<omega> args) \<in> range EInt" using insert(5) SumAux.prems(1) by (auto simp: type_restr_def args_def Let_def)
-    have aux1: "(\<And>a b. a \<in> (insert x F) \<Longrightarrow> b \<in> valid_sumaux_maps \<Longrightarrow> insert_sum args a b = insert_sum_comm args a b)" 
+    have y0_int: "snd (aggargs_\<omega> args) \<in> range EInt" using insert(5) SumAux.prems(1) by (auto simp: type_restr_def args_def)
+    have aux1: "(\<And>a b. a \<in> (Set.insert x F) \<Longrightarrow> b \<in> valid_sumaux_maps \<Longrightarrow> insert_sum args a b = insert_sum_comm args a b)" 
     proof -
       fix a b
-      assume a_def: "a \<in> (insert x F)" and b_def: "b \<in> valid_sumaux_maps"
-      have "meval_trm (aggargs_f args) a \<in> range EInt" using insert(5) a_def SumAux.prems(1) by(auto simp: type_restr_def Let_def args_def split:option.splits) (auto) 
+      assume a_def: "a \<in> (Set.insert x F)" and b_def: "b \<in> valid_sumaux_maps"
+      have "meval_trm (aggargs_f args) a \<in> range EInt" using insert(5) a_def SumAux.prems(1) by(auto simp: type_restr_def  args_def split:option.splits) (auto) 
       then show "insert_sum args a b = insert_sum_comm args a b" using y0_int b_def insert_sum_equiv[of args a b] by auto
     qed
-    moreover have aux2: "(\<And>a b. a \<in> (insert x F) \<Longrightarrow> b \<in> valid_sumaux_maps \<Longrightarrow> insert_sum_comm args a b \<in> valid_sumaux_maps)"
+    moreover have aux2: "(\<And>a b. a \<in> (Set.insert x F) \<Longrightarrow> b \<in> valid_sumaux_maps \<Longrightarrow> insert_sum_comm args a b \<in> valid_sumaux_maps)"
     proof -
       fix a b
-      assume "a \<in> (insert x F)" and "b \<in> valid_sumaux_maps"
+      assume "a \<in> (Set.insert x F)" and "b \<in> valid_sumaux_maps"
       then show "insert_sum_comm args a b \<in> valid_sumaux_maps"
         using y0_int 
-        apply(auto simp: valid_sumaux_maps_def  Let_def lookup_update' split:option.splits) 
-        by fastforce fastforce
+        apply(auto simp: valid_sumaux_maps_def lookup_update' split:option.splits) 
+        by fastforce+
     qed
-    moreover have valid_m: "m \<in> valid_sumaux_maps" using valid_maggaux_valid_map SumAux(1) by auto
-    ultimately have "Finite_Set.fold (insert_sum args) m (insert x F) = Finite_Set.fold (insert_sum_comm args) m (insert x F)"
-      using sumaux_finite_set_fold_eq[of "(insert x F)" "insert_sum args" "insert_sum_comm args" m] insert by auto
+    moreover have valid_m: "m \<in> valid_sumaux_maps" using valid_maggaux_valid_map SumAux(1) by blast
+    ultimately have "Finite_Set.fold (insert_sum args) m (Set.insert x F) = Finite_Set.fold (insert_sum_comm args) m (Set.insert x F)"
+      using sumaux_finite_set_fold_eq[of "(Set.insert x F)" "insert_sum args" "insert_sum_comm args" m] insert by auto
     moreover have "Finite_Set.fold (insert_sum args) m F = Finite_Set.fold (insert_sum_comm args) m F"
       using sumaux_finite_set_fold_eq[of F "insert_sum args" "insert_sum_comm args" m] using insert aux1 aux2 valid_m by auto
-    moreover have "Finite_Set.fold (insert_sum_comm args) m (insert x F) = insert_sum_comm args x (Finite_Set.fold (insert_sum_comm args) m F)"
+    moreover have "Finite_Set.fold (insert_sum_comm args) m (Set.insert x F) = insert_sum_comm args x (Finite_Set.fold (insert_sum_comm args) m F)"
       using  Finite_Set.comp_fun_commute.fold_insert[of "insert_sum_comm args" F x m] insert by auto
     moreover have "Finite_Set.fold (insert_sum args) m F \<in> valid_sumaux_maps" 
       using valid_maggaux_valid_map[of cols n g0 y \<omega> b f intermediate_map "X \<union> F"] intermediate_map_def' valid_int by(simp only:args_def)
     moreover have "meval_trm (aggargs_f args) x \<in> range EInt" 
-      using type_x SumAux.prems(1) by(auto simp: type_restr_def Let_def args_def split:option.splits)
-    ultimately have "Finite_Set.fold (insert_sum args) m (insert x F) = insert_sum args x (Finite_Set.fold (insert_sum args) m F)"
+      using type_x SumAux.prems(1) by(auto simp: type_restr_def args_def split:option.splits)
+    ultimately have "Finite_Set.fold (insert_sum args) m (Set.insert x F) = insert_sum args x (Finite_Set.fold (insert_sum args) m F)"
       using insert_sum_equiv[of args x "Finite_Set.fold (insert_sum args) m F"] y0_int by auto
-    then have "insert_maggaux args (insert x F) (SumAux m) = SumAux (insert_sum args x intermediate_map)"
+    then have "insert_maggaux args (Set.insert x F) (SumAux m) = SumAux (insert_sum args x intermediate_map)"
       using intermediate_map_def' by auto
-    then have "valid_maggaux args (insert_maggaux args (insert x F) (SumAux m)) (X \<union> insert x F)"
+    then have "valid_maggaux args (insert_maggaux args (Set.insert x F) (SumAux m)) (X \<union> Set.insert x F)"
       using valid_a by auto
     then show ?case by (simp only: args_def)
   qed
 next
-  case (MinAux x)
-  then show ?case sorry
-next
-  case (MaxAux x)
-  then show ?case sorry
-next
-  case (MedAux x)
+  case (RankAux x) 
   then show ?case sorry
 qed
 
-lemma valid_insert_maggaux: "valid_maggaux args aux X \<Longrightarrow> finite Y \<Longrightarrow>
+lemma valid_insert_maggaux': "valid_maggaux args aux X \<Longrightarrow> finite Y \<Longrightarrow>
     table (aggargs_b args + aggargs_n args) (aggargs_cols args) Y \<Longrightarrow>
     type_restr args Y \<Longrightarrow> X \<inter> Y = {} \<Longrightarrow>
     valid_maggaux args (insert_maggaux args Y aux) (X \<union> Y)"
   using valid_insert_maggaux_unfolded by (cases args) fast
+
+lemma valid_delete_sum_unfolded:
+  assumes valid_before: "valid_maggaux \<lparr>aggargs_cols = cols, aggargs_n = n, aggargs_g0 = g0, aggargs_y = y, aggargs_\<omega> = \<omega>, aggargs_b = b, aggargs_f = f\<rparr> (SumAux m) X" 
+  and in_set: "elem \<in> X"
+  and type_restr: "type_restr \<lparr>aggargs_cols = cols, aggargs_n = n, aggargs_g0 = g0, aggargs_y = y, aggargs_\<omega> = \<omega>, aggargs_b = b, aggargs_f = f\<rparr> {elem}"
+  shows "valid_maggaux \<lparr>aggargs_cols = cols, aggargs_n = n, aggargs_g0 = g0, aggargs_y = y, aggargs_\<omega> = \<omega>, aggargs_b = b, aggargs_f = f\<rparr> 
+        (SumAux (delete_sum \<lparr>aggargs_cols = cols, aggargs_n = n, aggargs_g0 = g0, aggargs_y = y, aggargs_\<omega> = \<omega>, aggargs_b = b, aggargs_f = f\<rparr> elem m)) (X - {elem})"
+proof - 
+  define updated_map where [simp]: "updated_map = delete_sum \<lparr>aggargs_cols = cols, aggargs_n = n, aggargs_g0 = g0, aggargs_y = y, aggargs_\<omega> = \<omega>, aggargs_b = b, aggargs_f = f\<rparr> elem m"
+  define updated_data where [simp]: "updated_data = X - {elem}"
+  interpret comp_fun_commute "\<lambda>(t, m) y. y + the_enat m" 
+    by(unfold_locales) auto
+  have len_commute: "comp_fun_commute (\<lambda>(t, m) y. y + the_enat m)" by unfold_locales
+  have plus'_comp_commute: "comp_fun_commute (\<lambda>(t, m) y. ((plus' t) ^^ (the_enat m)) y)"
+    using cmp_comm[of plus'] comp_fun_commute_plus' by(unfold_locales) auto
+  have valid_finite: "finite updated_data" using valid_before by auto
+  have valid_key_invariant: "\<And>k. k \<in> (drop b) ` updated_data \<longleftrightarrow> k \<in> Mapping.keys updated_map"
+  proof (rule iffI)
+    fix k
+    assume assm: "k \<in> (drop b) ` updated_data"
+    show "k \<in>  Mapping.keys updated_map"
+    proof(cases "drop b elem = k")
+      case True
+      then show ?thesis using length_flatten_multiset' assm valid_before 
+        apply(auto split:option.splits)
+        by (smt (z3) Set.member_filter card_eq_Suc_0_ex1 imageI in_set option.inject prod.inject) (smt (z3) Set.member_filter card_eq_Suc_0_ex1 imageI in_set option.inject prod.inject)
+    next
+      case False
+      then have "k \<in> (drop b) ` X" using assm valid_before by auto
+      then have "k \<in> Mapping.keys m" using valid_before by auto
+      then show ?thesis using False by(auto split:option.splits)
+    qed
+  next
+    fix k
+    assume assm: "k \<in> Mapping.keys updated_map"
+    then have in_map: "k \<in> Mapping.keys m" by(auto split:option.splits) (smt (z3) Diff_iff is_none_simps(2) keys_delete keys_is_none_rep lookup_update_neq)
+    then have in_set: "k \<in> (drop b) ` X" using valid_before by auto
+    show "k \<in> (drop b) ` updated_data"
+    proof(cases "drop b elem = k")
+      case True
+      then obtain l s where l_def: "Mapping.lookup m k = Some (l, s)" using in_map by (metis domIff keys_dom_lookup not_None_eq prod.exhaust_sel)
+      then have not_1: "l \<noteq> 1" using assm in_map True by(auto split:option.splits)
+      then have "l = length (flatten_multiset (group_multiset k b f X))" using l_def valid_before in_map by auto
+      then have "card (group k b X) \<noteq> 1" using length_flatten_multiset' valid_before not_1 by auto
+      moreover have "group k b X \<noteq> {}" using True assms by auto
+      ultimately obtain k' where "k' \<in> group k b X \<and> k' \<noteq> elem" by (metis is_singletonI' is_singleton_altdef)
+      then show ?thesis by auto
+    next
+      case False
+      then show ?thesis using in_set by auto
+    qed
+  qed
+  have valid_value_invariant: "\<And>k. k \<in> Mapping.keys updated_map \<longrightarrow> Mapping.lookup updated_map k = 
+          (let group = Set.filter (\<lambda>x. drop b x = k) updated_data;
+           M = (\<lambda>y. (y, ecard (Set.filter (\<lambda>x. meval_trm f x = y) group))) ` meval_trm f ` group;
+           M_list = flatten_multiset M;
+           aggtype = fst \<omega>;
+           y0 = (if aggtype = Formula.Agg_Sum then snd \<omega> else EInt 0)
+          in Some (length M_list, foldl plus y0 M_list))"
+  proof rule
+    fix k
+    define group where [simp]: "group = Set.filter (\<lambda>x. drop b x = k) updated_data"
+    define M where [simp]: "M = (\<lambda>y. (y, ecard (Set.filter (\<lambda>x. meval_trm f x = y) group))) ` meval_trm f ` group"
+    define old_group where [simp]: "old_group = Set.filter (\<lambda>x. drop b x = k) X"
+    define old_M where [simp]: "old_M = (\<lambda>y. (y, ecard (Set.filter (\<lambda>x. meval_trm f x = y) old_group))) ` meval_trm f ` old_group"
+    define old_evals where "old_evals = meval_trm f ` old_group"
+    define y0 where [simp]: "y0 = (if fst \<omega>  = Formula.Agg_Sum then snd \<omega> else EInt 0)"
+    define term' where [simp]: "term' = meval_trm f elem"
+    assume assm: "k \<in> Mapping.keys updated_map"
+    then have in_old: "k \<in> Mapping.keys m" by(auto split:option.splits) (smt (z3) Diff_iff insert_iff is_none_simps(2) keys_delete keys_is_none_rep keys_update)
+    have multiset_int: "\<And>t m. (t, m) \<in> M \<Longrightarrow> t \<in> range EInt" using type_restr valid_before by (auto simp: type_restr_def image_subset_iff)  
+    then have M_int: "set (flatten_multiset M) \<subseteq> range EInt" using flatten_multiset_eint[of M]  valid_finite by auto
+    have old_multiset_int: "\<And>t m. (t, m) \<in> old_M \<Longrightarrow> t \<in> range EInt" using type_restr valid_before by (auto simp: type_restr_def image_subset_iff)  
+    then have M_old_int: "set (flatten_multiset old_M) \<subseteq> range EInt" using flatten_multiset_eint[of old_M] finite valid_before by auto
+    have y0_int: "y0 \<in> range EInt" using type_restr valid_before by (auto simp: type_restr_def)
+    have both_finite: "finite M \<and> finite old_M" using valid_finite by auto
+    show "Mapping.lookup updated_map k = 
+          (let group = Set.filter (\<lambda>x. drop b x = k) updated_data;
+           M = (\<lambda>y. (y, ecard (Set.filter (\<lambda>x. meval_trm f x = y) group))) ` meval_trm f ` group;
+           M_list = flatten_multiset M;
+           aggtype = fst \<omega>;
+           y0 = (if aggtype = Formula.Agg_Sum then snd \<omega> else EInt 0)
+          in Some (length M_list, foldl plus y0 M_list))"
+    proof(cases "drop b elem = k")
+      case True
+      then have grp_def: "group = Set.remove elem old_group" by auto
+      have elem_group: "drop b elem = k" using True by auto
+      have "length(flatten_multiset(M)) = card group" using length_flatten_multiset' valid_before
+        by(simp only: M_def old_M_def group_multiset_def Let_def) (auto)
+      moreover have "length(flatten_multiset(old_M)) = card old_group" using length_flatten_multiset' valid_before
+        by(simp only: M_def old_M_def group_multiset_def Let_def) (auto)
+      ultimately have len: "length(flatten_multiset(M)) = length(flatten_multiset(old_M)) - 1" using grp_def in_set
+        by(auto) (smt (z3) One_nat_def Set.member_filter Set.remove_def True card_Diff_singleton finite_filter valid_before valid_maggaux.simps)
+      obtain len sum where ls_def: "Mapping.lookup m k = Some (len, sum)" using in_old by (metis domIff keys_dom_lookup not_Some_eq prod.exhaust_sel)
+      then have l_def: "len = length(flatten_multiset(old_M))" using valid_before in_old by auto
+      have len_not_1: "len \<noteq> 1" using assm ls_def elem_group by(auto split:option.splits)
+      have s_def: "sum = foldl plus y0 (flatten_multiset old_M)" using ls_def valid_before in_old by auto
+      have "foldl plus y0 (flatten_multiset M) = (foldl plus y0 (flatten_multiset old_M)) - term'"
+      proof(cases "Set.filter (\<lambda>x. meval_trm f x = meval_trm f elem) old_group = {elem}")
+        case True
+        have "group_multiset k b f (X - {elem}) = group_multiset k b f X - {(meval_trm f elem, 1)}"
+          using multiset_single_term_remove elem_group True by auto
+        then have M_remove_def: "M = old_M - {(meval_trm f elem, 1)}" by simp
+        have in_M: "(meval_trm f elem, 1) \<in> old_M" using single_term_in_multiset True elem_group by auto
+        have fold_eq1: "foldl (+) y0 (flatten_multiset M) = Finite_Set.fold (\<lambda>(t, m). (plus') t ^^ the_enat m) y0 M"
+          using foldl_flatten_multiset foldl_eint_equival M_int y0_int both_finite comm_plus' comp_fun_commute_plus' by(simp)
+        have fold_eq2: "foldl (+) y0 (flatten_multiset old_M) = Finite_Set.fold (\<lambda>(t, m). (plus') t ^^ the_enat m) y0 old_M" 
+          using foldl_flatten_multiset foldl_eint_equival M_old_int y0_int both_finite comm_plus' comp_fun_commute_plus' by simp
+        have "Finite_Set.fold (\<lambda>(t, m). plus' t ^^ the_enat m) y0 (Set.insert (meval_trm f elem, 1) (old_M - {(meval_trm f elem, 1)})) =
+              (plus' term' ^^ 1) (Finite_Set.fold (\<lambda>(t, m). plus' t ^^ the_enat m) y0 (old_M - {(meval_trm f elem, 1)} - {(meval_trm f elem, 1)}))"
+          using Finite_Set.comp_fun_commute.fold_insert_remove[of "\<lambda>(t, m). (plus') t ^^ the_enat m" "old_M - {(meval_trm f elem, 1)}" y0 "(meval_trm f elem, 1)"]
+            plus'_comp_commute M_remove_def by(simp) (smt (z3) finite_filter finite_imageI plus'_iter_one_enat valid_before valid_maggaux.elims(2))
+        then have aux: "Finite_Set.fold (\<lambda>(t, m). (plus') t ^^ the_enat m) y0 old_M = (plus' term' ^^ 1) (Finite_Set.fold (\<lambda>(t, m). (plus') t ^^ the_enat m) y0 M)"
+          using in_M by (metis Diff_idemp M_remove_def insert_Diff)
+        moreover have fold_eint: "(Finite_Set.fold (\<lambda>(t, m). (plus') t ^^ the_enat m) y0 M) \<in> range EInt"  using both_finite finite_set_fold_int multiset_int y0_int by blast
+        moreover have term'_eint: "term' \<in> range EInt" using in_M old_multiset_int term'_def by blast
+        ultimately have "Finite_Set.fold (\<lambda>(t, m). (plus') t ^^ the_enat m) y0 M = (minus' term' ^^ 1) (Finite_Set.fold (\<lambda>(t, m). (plus') t ^^ the_enat m) y0 old_M)"
+          using plus'_minus'_id by auto
+        then have "Finite_Set.fold (\<lambda>(t, m). (plus') t ^^ the_enat m) y0 M = (Finite_Set.fold (\<lambda>(t, m). (plus') t ^^ the_enat m) y0 old_M) - term'" 
+        by (metis fold_eint aux term'_eint iter_plus'_int minus'_iter_one_enat minus_minus'_equiv one_enat_def term'_def the_enat.simps)
+        then show ?thesis using fold_eq1 fold_eq2 by auto
+      next
+        case False
+        then obtain y where y_def: "(meval_trm f elem, y) \<in> old_M" using elem_group in_set by fastforce
+        then obtain i where i_def: "y = enat i" by (smt (z3) Pair_inject ecard_def finite_filter image_iff old_M_def old_group_def valid_before valid_maggaux.simps)
+        have "Set.filter (\<lambda>x. meval_trm f x = meval_trm f elem) (Set.filter (\<lambda>x. drop b x = drop b elem) X) \<noteq> {}" using in_set by force
+        then have i_not_zero: "i \<noteq> 0" using y_def by(auto) (smt (z3) Set.member_filter card_eq_0_iff ecard_def enat_0_iff(2) finite.emptyI finite.insertI finite_Diff2 finite_filter i_def insert_absorb insert_not_empty updated_data_def valid_finite)
+        then obtain i' where i'_def: "i' = i - 1" by auto
+        then have i'_aux: "i' + 1 = i" using i_not_zero by auto
+        have finite_remove: "finite (old_M - {(meval_trm f elem, y)})" using both_finite finite_Diff  by (auto simp: Set.remove_def)
+        have finite_insert: "finite (Set.insert (meval_trm f elem, y) old_M)" using both_finite by blast
+        have "finite X" using valid_before by auto
+        moreover have "Set.filter (\<lambda>x. meval_trm f x = meval_trm f elem) (Optimized_Agg.group k b X) \<noteq> {elem}" using False by auto
+        ultimately have "group_multiset k b f (X - {elem}) = Set.insert (meval_trm f elem, y - 1) (group_multiset k b f X - {(meval_trm f elem, y)})"
+          using multiset_multiple_term_remove elem_group in_set False y_def by simp
+        then have M_insert_remove_def: "M = Set.insert (meval_trm f elem, y - 1) (old_M - {(meval_trm f elem, y)})" 
+          by simp
+        have foldl_plus_plus'_equiv: "foldl (+) y0 (flatten_multiset M) = foldl (plus') y0 (flatten_multiset M)" using foldl_eint_equival M_int y0_int by auto
+        have aux1: "foldl (plus') y0 (flatten_multiset (Set.insert (term', y) old_M)) = Finite_Set.fold (\<lambda>(t, m). (plus') t ^^ the_enat m) y0 (Set.insert (term', y) old_M)"
+          using foldl_flatten_multiset[of "Set.insert (term', y) old_M" plus' y0] finite_insert comp_fun_commute_plus' comm_plus' by auto
+        moreover have foldl_remove_equiv: "foldl plus' y0 (flatten_multiset(old_M - {(term', y)})) = Finite_Set.fold (\<lambda>(t, m). (plus') t ^^ the_enat m) y0 (old_M - {(term', y)})"
+          using foldl_flatten_multiset[of "old_M - {(term', y)}" plus' y0] finite_insert comp_fun_commute_plus' comm_plus' by auto
+        ultimately have aux: "foldl plus' y0 (flatten_multiset(Set.insert (term', y) old_M)) = ((plus' term') ^^ (the_enat y)) (foldl plus' y0 (flatten_multiset(old_M - {(term', y)})))" 
+          using  finite_insert plus'_comp_commute Finite_Set.comp_fun_commute.fold_insert_remove[of "\<lambda>(t, m). (plus') t ^^ the_enat m"] by auto
+        moreover have term'_int: "term' \<in> range EInt" using old_multiset_int term'_def y_def by blast
+        moreover have "foldl plus' y0 (flatten_multiset(old_M - {(term', y)})) \<in> range EInt" 
+          using foldl_remove_equiv by (metis DiffD1 finite_remove finite_set_fold_int old_multiset_int term'_def y0_int)
+        ultimately have aux: "foldl plus' y0 (flatten_multiset(old_M - {(term', y)})) = ((minus' term') ^^ (the_enat y)) (foldl plus' y0 (flatten_multiset(old_M)))"
+          using plus'_minus'_id by (metis comp_apply insert_absorb term'_def y_def)
+        moreover have "(term', y - 1) \<notin> old_M - {(term', y)}" using y_def by auto
+        ultimately have "Finite_Set.fold (\<lambda>(t, m). (plus') t ^^ the_enat m) y0 M = ((plus' term') ^^ i') (((minus' term') ^^ (i' + 1)) (foldl plus' y0 (flatten_multiset(old_M))))"
+          using Finite_Set.comp_fun_commute.fold_insert[of "\<lambda>(t, m). plus' t ^^ the_enat m"] plus'_comp_commute finite_remove i_def i'_def i'_aux
+          by(simp only: M_insert_remove_def term'_def) (metis (no_types, lifting) foldl_remove_equiv idiff_enat_enat old.prod.case one_enat_def term'_def the_enat.simps)
+        moreover have "foldl (plus') y0 (flatten_multiset(M)) = Finite_Set.fold (\<lambda>(t, m). (plus') t ^^ the_enat m) y0 M"
+          using foldl_flatten_multiset[of M plus' y0] both_finite comp_fun_commute_plus' comm_plus' by auto
+        ultimately have "foldl (plus') y0 (flatten_multiset(M)) = minus' term' (foldl plus' y0 (flatten_multiset(old_M)))"
+          using aux1 plus'_minus'_minus by (metis both_finite comp_eq_dest_lhs finite_set_fold_int insert_absorb old_multiset_int term'_def y0_int y_def)
+        moreover have "foldl plus' y0 (flatten_multiset(old_M)) \<in> range EInt" 
+          by (metis aux1 both_finite finite_set_fold_int insert_absorb old_multiset_int term'_def y0_int y_def)
+        ultimately show ?thesis using M_old_int foldl_eint_equival foldl_plus_plus'_equiv minus_minus'_equiv term'_int y0_int by auto
+      qed
+      moreover have "Mapping.lookup updated_map k = Some (len - 1, sum - term')" using ls_def elem_group len_not_1
+        by(auto simp: lookup_update split:option.splits) 
+      ultimately show ?thesis using len l_def s_def by auto
+    next
+      case False
+      then have "group = old_group" by auto
+      moreover have "Mapping.lookup updated_map k = Mapping.lookup m k" using False 
+        by(auto simp: lookup_update' split:option.splits) (metis lookup_update' update_delete)
+      ultimately show ?thesis using valid_before in_old by auto
+    qed
+  qed
+  have "type_restr \<lparr>aggargs_cols = cols, aggargs_n = n, aggargs_g0 = g0, aggargs_y = y, aggargs_\<omega> = \<omega>, aggargs_b = b, aggargs_f = f\<rparr> X"
+    using valid_before by auto
+  then have valid_type_restr: "type_restr \<lparr>aggargs_cols = cols, aggargs_n = n, aggargs_g0 = g0, aggargs_y = y, aggargs_\<omega> = \<omega>, aggargs_b = b, aggargs_f = f\<rparr> (X - {elem})"
+    using valid_before by (auto simp: type_restr_def) blast+
+  show ?thesis using valid_value_invariant valid_key_invariant valid_finite valid_before valid_type_restr
+    by auto
+qed
+
+lemma valid_delete_cnt_unfolded: 
+  assumes valid_before: "valid_maggaux \<lparr>aggargs_cols = cols, aggargs_n = n, aggargs_g0 = g0, aggargs_y = y, aggargs_\<omega> = \<omega>, aggargs_b = b, aggargs_f = f\<rparr> (CntAux m) X" 
+  and in_set: "elem \<in> X"
+  shows "valid_maggaux \<lparr>aggargs_cols = cols, aggargs_n = n, aggargs_g0 = g0, aggargs_y = y, aggargs_\<omega> = \<omega>, aggargs_b = b, aggargs_f = f\<rparr> 
+        (CntAux (delete_cnt \<lparr>aggargs_cols = cols, aggargs_n = n, aggargs_g0 = g0, aggargs_y = y, aggargs_\<omega> = \<omega>, aggargs_b = b, aggargs_f = f\<rparr> elem m)) (X - {elem})"
+proof - 
+  define updated_map where [simp]: "updated_map = delete_cnt \<lparr>aggargs_cols = cols, aggargs_n = n, aggargs_g0 = g0, aggargs_y = y, aggargs_\<omega> = \<omega>, aggargs_b = b, aggargs_f = f\<rparr> elem m"
+  define updated_data where [simp]: "updated_data = X - {elem}"
+  interpret comp_fun_commute "\<lambda>(t, m) y. y + the_enat m" 
+    by(unfold_locales) auto
+  have valid_finite: "finite updated_data" using valid_before by auto
+  have valid_key_invariant: "\<And>k. k \<in> (drop b) ` updated_data \<longleftrightarrow> k \<in> Mapping.keys updated_map"
+  proof (rule iffI)
+    fix k
+    assume assm: "k \<in> (drop b) ` updated_data"
+    show "k \<in>  Mapping.keys updated_map"
+    proof(cases "drop b elem = k")
+      case True
+      then show ?thesis using length_flatten_multiset' assm valid_before 
+        by(auto split:option.splits) (smt (z3) Set.member_filter card_eq_Suc_0_ex1 in_set is_none_simps(2) keys_is_none_rep option.inject)
+    next
+      case False
+      then show ?thesis 
+        using valid_before assm
+        by(auto simp only: updated_map_def delete_cnt.simps Let_def updated_data_def split:option.splits) auto
+    qed
+  next
+    fix k
+    assume assm: "k \<in> Mapping.keys updated_map"
+    show "k \<in> (drop b) ` updated_data"
+    proof (cases "k \<in> Mapping.keys m")
+      case True
+      then show ?thesis using length_flatten_multiset' assm valid_before 
+        apply(auto split:option.splits) by(fastforce) (smt (z3) Diff_iff Set.member_filter card_eq_Suc_0_ex1 empty_iff image_iff insert_iff keys_delete option.sel)
+    next
+      case False
+      then show ?thesis using valid_before assm
+        by(auto) (smt (verit, best) imageI in_set insertCI insert_Diff insert_absorb keys_delete keys_update option.simps(5))
+    qed 
+  qed
+  have valid_value_invariant: "\<And>k. k \<in> Mapping.keys updated_map \<longrightarrow> Mapping.lookup updated_map k = 
+          (let group = Set.filter (\<lambda>x. drop b x = k) updated_data;
+           M = (\<lambda>y. (y, ecard (Set.filter (\<lambda>x. meval_trm f x = y) group))) ` meval_trm f ` group
+          in Some (length (flatten_multiset M)))"
+  proof rule
+    fix k
+    define group where [simp]: "group = Set.filter (\<lambda>x. drop b x = k) updated_data"
+    define M where [simp]: "M = (\<lambda>y. (y, ecard (Set.filter (\<lambda>x. meval_trm f x = y) group))) ` meval_trm f ` group"
+    define old_group where [simp]: "old_group = Set.filter (\<lambda>x. drop b x = k) X"
+    define old_M where [simp]: "old_M = (\<lambda>y. (y, ecard (Set.filter (\<lambda>x. meval_trm f x = y) old_group))) ` meval_trm f ` old_group"
+    define old_evals where "old_evals = meval_trm f ` old_group"
+    assume assm: "k \<in> Mapping.keys updated_map"
+    then have in_old: "k \<in> Mapping.keys m" by(auto split:option.splits) (smt (z3) Diff_iff insert_iff is_none_simps(2) keys_delete keys_is_none_rep keys_update)
+    show "Mapping.lookup updated_map k = 
+          (let group = Set.filter (\<lambda>x. drop b x = k) updated_data;
+           M = (\<lambda>y. (y, ecard (Set.filter (\<lambda>x. meval_trm f x = y) group))) ` meval_trm f ` group
+          in Some (length (flatten_multiset M)))"
+    proof(cases "drop b elem = k")
+      case True
+      then have grp_def: "group = Set.remove elem old_group" by auto
+      have "length(flatten_multiset(M)) = card group" using length_flatten_multiset' valid_before
+        by(simp only: M_def old_M_def group_multiset_def Let_def) (auto)
+      moreover have "length(flatten_multiset(old_M)) = card old_group" using length_flatten_multiset' valid_before
+        by(simp only: M_def old_M_def group_multiset_def Let_def) (auto)
+      ultimately have len: "length(flatten_multiset(M)) = length(flatten_multiset(old_M)) - 1" using grp_def in_set
+        by(auto) (smt (z3) One_nat_def Set.member_filter Set.remove_def True card_Diff_singleton finite_filter valid_before valid_maggaux.simps)
+      obtain i where i_def: "Mapping.lookup m k = Some i" using in_old by (metis default_def lookup_default)
+      then have i_def': "i = length(flatten_multiset(old_M))" using valid_before in_old by auto
+      then have "Mapping.lookup updated_map k = Some (i - 1)" using True assm i_def by(auto simp: lookup_update split:option.splits)
+      then show ?thesis using len i_def' by(simp) 
+    next
+      case False
+      then have "group = old_group" by auto
+      moreover have "Mapping.lookup updated_map k = Mapping.lookup m k" using False 
+        by(auto simp: lookup_update' split:option.splits) (metis lookup_update' update_delete)
+      ultimately show ?thesis using valid_before in_old by auto
+    qed
+  qed
+  show ?thesis using valid_value_invariant valid_key_invariant valid_finite valid_before
+    by auto
+qed
+
+lemma valid_delete_maggaux_unfolded: 
+  "valid_maggaux \<lparr>aggargs_cols = cols, aggargs_n = n, aggargs_g0 = g0, aggargs_y = y, aggargs_\<omega> = \<omega>, aggargs_b = b, aggargs_f = f\<rparr> aux X \<Longrightarrow>
+  Y \<subseteq> X  \<Longrightarrow>
+  valid_maggaux \<lparr>aggargs_cols = cols, aggargs_n = n, aggargs_g0 = g0, aggargs_y = y, aggargs_\<omega> = \<omega>, aggargs_b = b, aggargs_f = f\<rparr> 
+  (delete_maggaux \<lparr>aggargs_cols = cols, aggargs_n = n, aggargs_g0 = g0, aggargs_y = y, aggargs_\<omega> = \<omega>, aggargs_b = b, aggargs_f = f\<rparr> Y aux) (X - Y)" 
+proof(induction aux)
+  case (CntAux m)
+  have subset: "Y \<subseteq> X" using CntAux by auto
+  have finite_y: "finite Y" using CntAux rev_finite_subset by auto
+  then show ?case using subset
+  proof(induction Y)
+    case empty
+    then show ?case using CntAux by auto
+  next
+    case (insert x F)
+    define args where "args = \<lparr>aggargs_cols = cols, aggargs_n = n, aggargs_g0 = g0, aggargs_y = y, aggargs_\<omega> = \<omega>, aggargs_b = b, aggargs_f = f\<rparr>"
+    interpret comp_fun_commute "delete_cnt args"
+      using delete_cnt_comm by unfold_locales auto
+    obtain intermediate_map where intermediate_map_def: "CntAux intermediate_map = delete_maggaux args F (CntAux m)" by auto
+    have valid_a: "valid_maggaux args (CntAux (delete_cnt args x intermediate_map)) (X - F - {x})" 
+      using valid_delete_cnt_unfolded[of cols n g0 y \<omega> b f intermediate_map "X - F" x] insert args_def intermediate_map_def by(auto)
+    then have "Finite_Set.fold (delete_cnt args) m (Set.insert x F) = delete_cnt args x (Finite_Set.fold (delete_cnt args) m F)"
+      using Finite_Set.comp_fun_commute.fold_insert insert by auto
+    moreover have "CntAux (Finite_Set.fold (delete_cnt args) m F) = CntAux intermediate_map"
+      by(auto simp:intermediate_map_def)
+    ultimately have "delete_maggaux args (Set.insert x F) (CntAux m) = CntAux (delete_cnt args x intermediate_map)"
+      using  Finite_Set.comp_fun_commute.fold_insert by auto
+    then have "valid_maggaux args (delete_maggaux args (Set.insert x F) (CntAux m)) (X - Set.insert x F)"
+      using valid_a by (metis Diff_insert)
+    then show ?case
+      by (auto simp: args_def)
+  qed
+next
+  case (SumAux m)
+  have subset: "Y \<subseteq> X" using SumAux by auto
+  have valid_before: "valid_maggaux \<lparr>aggargs_cols = cols, aggargs_n = n, aggargs_g0 = g0, aggargs_y = y, aggargs_\<omega> = \<omega>, aggargs_b = b, aggargs_f = f\<rparr> (SumAux m) X" using SumAux by auto
+  have finite_y: "finite Y" using subset valid_before finite_subset by auto
+  then show ?case using subset 
+  proof(induction Y)
+    case empty
+    then show ?case using SumAux by auto
+  next
+    case (insert x F)
+    define args where "args = \<lparr>aggargs_cols = cols, aggargs_n = n, aggargs_g0 = g0, aggargs_y = y, aggargs_\<omega> = \<omega>, aggargs_b = b, aggargs_f = f\<rparr>"
+    interpret comp_fun_commute "delete_sum_comm args"
+      using delete_sum_comm by unfold_locales auto
+    have x_in_X: "x \<in> X" using insert by auto
+    obtain intermediate_map where intermediate_map_def: "SumAux intermediate_map = delete_maggaux args F (SumAux m)" by auto
+    then have intermediate_map_def': "intermediate_map = Finite_Set.fold (delete_sum args) m F" by auto
+    have F_subs: "F \<subseteq> X" using insert(4) by auto
+    moreover have "valid_maggaux args (SumAux m) X" using valid_before by (auto simp:args_def)
+    ultimately have valid_int: "valid_maggaux args (SumAux intermediate_map) (X - F)" using insert(3) by(simp only:intermediate_map_def args_def)
+    moreover have "x \<in> X - F" using insert(2) insert.prems(1) by auto
+    moreover have type_x: "type_restr args {x}" using valid_before x_in_X apply (cases "fst \<omega>") apply(auto simp: args_def type_restr_def) by blast blast
+    ultimately have valid_a: "valid_maggaux args (SumAux (delete_sum args x intermediate_map)) (X - F - {x})" 
+      using valid_delete_sum_unfolded using args_def by blast
+    have y0_int: "snd (aggargs_\<omega> args) \<in> range EInt" using valid_before SumAux.prems(1) by (auto simp: type_restr_def args_def)
+    have aux1: "(\<And>a b. a \<in> (Set.insert x F) \<Longrightarrow> b \<in> valid_sumaux_maps \<Longrightarrow> delete_sum args a b = delete_sum_comm args a b)" 
+    proof -
+      fix a b
+      assume a_def: "a \<in> (Set.insert x F)" and b_def: "b \<in> valid_sumaux_maps"
+      have "meval_trm (aggargs_f args) a \<in> range EInt" using valid_before a_def SumAux.prems(1) x_in_X insert(4) F_subs
+        apply(auto simp: type_restr_def  args_def split:option.splits) apply(auto) by blast blast
+      then show "delete_sum args a b = delete_sum_comm args a b" using y0_int b_def delete_sum_equiv[of args a b] by auto
+    qed
+    moreover have aux2: "(\<And>a b. a \<in> (Set.insert x F) \<Longrightarrow> b \<in> valid_sumaux_maps \<Longrightarrow> delete_sum_comm args a b \<in> valid_sumaux_maps)"
+    proof -
+      fix a b
+      assume "a \<in> (Set.insert x F)" and "b \<in> valid_sumaux_maps"
+      then show "delete_sum_comm args a b \<in> valid_sumaux_maps"
+        using y0_int 
+        apply(auto simp: valid_sumaux_maps_def lookup_update' split:option.splits) 
+        apply (metis Diff_iff insert_iff is_none_simps(2) keys_delete keys_is_none_rep lookup_update' update_delete)
+        using minus'.simps(1) apply blast
+        apply (metis Diff_iff insertI1 is_none_simps(2) keys_delete keys_is_none_rep lookup_update' update_delete)
+        using minus'.simps(1) by blast
+    qed
+    moreover have valid_m: "m \<in> valid_sumaux_maps" using valid_maggaux_valid_map SumAux(1) by blast
+    ultimately have "Finite_Set.fold (delete_sum args) m (Set.insert x F) = Finite_Set.fold (delete_sum_comm args) m (Set.insert x F)"
+      using sumaux_finite_set_fold_eq[of "(Set.insert x F)" "delete_sum args" "delete_sum_comm args" m] insert by auto
+    moreover have "Finite_Set.fold (delete_sum args) m F = Finite_Set.fold (delete_sum_comm args) m F"
+      using sumaux_finite_set_fold_eq[of F "delete_sum args" "delete_sum_comm args" m] using insert aux1 aux2 valid_m by auto
+    moreover have "Finite_Set.fold (delete_sum_comm args) m (Set.insert x F) = delete_sum_comm args x (Finite_Set.fold (delete_sum_comm args) m F)"
+      using  Finite_Set.comp_fun_commute.fold_insert[of "delete_sum_comm args" F x m] insert by auto
+    moreover have "Finite_Set.fold (delete_sum args) m F \<in> valid_sumaux_maps" 
+      using valid_maggaux_valid_map[of cols n g0 y \<omega> b f intermediate_map "X - F"] intermediate_map_def' valid_int by(simp only:args_def)
+    moreover have "meval_trm (aggargs_f args) x \<in> range EInt" 
+      using type_x SumAux.prems(1) by(auto simp: type_restr_def args_def split:option.splits)
+    ultimately have "Finite_Set.fold (delete_sum args) m (Set.insert x F) = delete_sum args x (Finite_Set.fold (delete_sum args) m F)"
+      using insert_sum_equiv[of args x "Finite_Set.fold (delete_sum args) m F"] y0_int delete_sum_equiv by auto
+    then have "delete_maggaux args (Set.insert x F) (SumAux m) = SumAux (delete_sum args x intermediate_map)"
+      using intermediate_map_def' by auto
+    then have "valid_maggaux args (delete_maggaux args (Set.insert x F) (SumAux m)) (X - Set.insert x F)"
+      using valid_a by (metis Diff_insert)
+    then show ?case by (simp only: args_def)
+  qed
+next
+  case (RankAux x)
+  then show ?case sorry
+qed
+
+lemma valid_delete_maggaux': "valid_maggaux args aux X \<Longrightarrow>
+    table (aggargs_b args + aggargs_n args) (aggargs_cols args) Y \<Longrightarrow> Y \<subseteq> X \<Longrightarrow>
+    valid_maggaux args (delete_maggaux args Y aux) (X - Y)"
+  using valid_delete_maggaux_unfolded by (cases args) blast
 
 lemma valid_aggmap_empty_data: "valid_aggmap g b f m X \<Longrightarrow> X = {} \<longleftrightarrow> Mapping.keys m = {}"
   by auto
@@ -949,16 +1647,16 @@ proof -
   define M_list where [simp]: "M_list = linorder.sorted_list_of_set (le_of_comp c) M"
   obtain elem where elem_prop: "elem \<in> X \<and> drop b elem = k" using in_map valid_map imageE[of k "drop b" X] by auto
   then obtain m where m_prop: "(meval_trm f elem, m) \<in> M" 
-    by (auto simp: Let_def) fastforce
+    by auto fastforce
   define group where [simp]: "group = Set.filter (\<lambda>x. meval_trm f x = meval_trm f elem) (Set.filter (\<lambda>x. drop b x = k) X)"
   have "ecard group \<noteq> 0" using finite elem_prop by (auto simp:ecard_def zero_enat_def) 
   then have m_pos: "m > 0 \<and> m \<noteq> \<infinity>" 
-    using elem_prop m_prop finite  by (auto simp: Let_def ecard_def)
+    using elem_prop m_prop finite  by (auto simp: ecard_def)
   then have "the_enat m > 0"
     apply(auto simp: the_enat_def)
     using enat_0_iff(1) by blast
   then obtain n where n_def: "the_enat m = Suc n" using gr0_implies_Suc by auto
-  have finite_m: "finite M" using finite by (auto simp: Let_def)
+  have finite_m: "finite M" using finite by auto
   then have "(meval_trm f elem, m) \<in> set (linorder.sorted_list_of_set (le_of_comp c) M)"
     using m_prop linorder.set_sorted_list_of_set[OF c_class] by auto
   then show ?thesis 
@@ -992,11 +1690,11 @@ proof(induction aux)
       define group where [simp]: "group = Set.filter (\<lambda>x. drop b x = k) X"
       define M where [simp]: "M = (\<lambda>y. (y, ecard (Set.filter (\<lambda>x. meval_trm f x = y) group))) ` meval_trm f ` group"
       have "Mapping.lookup m k = Some (length (flatten_multiset M), foldl plus (snd \<omega>) (flatten_multiset M))" 
-        using SumAux k_assm True by (simp add: Let_def lookup_default_def)
+        using SumAux k_assm True by (simp add: lookup_default_def)
       then have "result = k[y:= Some (eval_agg_op \<omega> M)]" 
         using k_assm True by auto (metis (no_types, lifting) eval_agg_op.simps(4) prod.exhaust_sel)
       then show "result \<in> eval_aggargs \<lparr>aggargs_cols = cols, aggargs_n = n, aggargs_g0 = g0, aggargs_y = y, aggargs_\<omega> = \<omega>, aggargs_b = b, aggargs_f = f\<rparr> X"
-        using k_assm SumAux by (auto simp add: Let_def eval_agg_def eval_aggargs_def)
+        using k_assm SumAux by (auto simp add: eval_agg_def eval_aggargs_def)
     next
       fix result
       assume "result \<in> eval_aggargs \<lparr>aggargs_cols = cols, aggargs_n = n, aggargs_g0 = g0, aggargs_y = y, aggargs_\<omega> = \<omega>, aggargs_b = b, aggargs_f = f\<rparr> X"
@@ -1007,9 +1705,9 @@ proof(induction aux)
       define group where [simp]: "group = Set.filter (\<lambda>x. drop b x = k) X"
       define M where [simp]: "M = (\<lambda>y. (y, ecard (Set.filter (\<lambda>x. meval_trm f x = y) group))) ` meval_trm f ` group"
       have key_in_map: "k \<in> Mapping.keys m"
-        using SumAux by auto (metis k_assm)
+        using SumAux apply(auto) using k_assm by presburger+
       then have "Mapping.lookup m k = Some (length (flatten_multiset M), foldl plus (snd \<omega>) (flatten_multiset M))"
-        using SumAux True by (simp add: Let_def lookup_default_def)
+        using SumAux True by (simp add: lookup_default_def)
       then have "result = (case Mapping.lookup m k of 
                             Some (_, agg_sum) \<Rightarrow> k[y:=Some agg_sum]
                           | None \<Rightarrow> k)"
@@ -1033,14 +1731,14 @@ proof(induction aux)
       define M where [simp]: "M = (\<lambda>y. (y, ecard (Set.filter (\<lambda>x. meval_trm f x = y) group))) ` meval_trm f ` group"
       have not_empty: "flatten_multiset M \<noteq> []" 
         using flatten_multiset_not_empty[of _ b f m X k] SumAux k_assm False 
-        by (auto simp: Let_def) force
+        by auto
       have "Mapping.lookup m k = Some (length (flatten_multiset M), foldl plus (EInt 0) (flatten_multiset M))" 
-        using SumAux k_assm agg_type by (simp add: Let_def lookup_default_def)
+        using SumAux k_assm agg_type by (simp add: lookup_default_def)
       then have "result = k[y:= Some (eval_agg_op \<omega> M)]" 
         using k_assm agg_type not_empty SumAux aux_def
-        by(auto simp add: Let_def split:list.splits)
+        by(auto split:list.splits)
       then show "result \<in> eval_aggargs \<lparr>aggargs_cols = cols, aggargs_n = n, aggargs_g0 = g0, aggargs_y = y, aggargs_\<omega> = \<omega>, aggargs_b = b, aggargs_f = f\<rparr> X"
-        using k_assm SumAux by (auto simp add: Let_def eval_agg_def eval_aggargs_def)
+        using k_assm SumAux by (auto simp add: eval_agg_def eval_aggargs_def)
     next
       fix result
       assume "result \<in> eval_aggargs \<lparr>aggargs_cols = cols, aggargs_n = n, aggargs_g0 = g0, aggargs_y = y, aggargs_\<omega> = \<omega>, aggargs_b = b, aggargs_f = f\<rparr> X"
@@ -1050,34 +1748,27 @@ proof(induction aux)
         unfolding eval_aggargs_def eval_agg_def empty_table_def using assm_reg by auto
       define group where [simp]: "group = Set.filter (\<lambda>x. drop b x = k) X"
       define M where [simp]: "M = (\<lambda>y. (y, ecard (Set.filter (\<lambda>x. meval_trm f x = y) group))) ` meval_trm f ` group"
-      have "k \<in> Mapping.keys m" using k_assm SumAux 
-      by (metis (no_types, lifting) aggaux.simps(27) valid_aggmap_def valid_maggaux.simps)
+      have "k \<in> Mapping.keys m" using k_assm SumAux by auto
       then have not_empty: "flatten_multiset M \<noteq> []" 
         using flatten_multiset_not_empty[of _ b f m X k] SumAux k_assm False 
         unfolding group_multiset_def Let_def M_def group_def by fastforce
       have key_in_map: "k \<in> Mapping.keys m"
-        using SumAux by auto (metis k_assm)
+        using SumAux \<open>k \<in> Mapping.keys m\<close> by force
       then have "Mapping.lookup m k = Some (length (flatten_multiset M), foldl plus (EInt 0) (flatten_multiset M))"
-        using SumAux False by (simp add: Let_def lookup_default_def)
+        using SumAux False by (simp add: lookup_default_def)
       then have "result = (case Mapping.lookup m k of 
                              Some (cnt, agg_sum) \<Rightarrow> k[y:=Some (EFloat ((double_of_event_data agg_sum) / (double_of_int cnt)))]
                           | None \<Rightarrow> k)"
         using False k_assm not_empty aux_def unfolding M_def group_def 
-        by(auto simp: Let_def split:list.splits)
+        by(auto split:list.splits)
       then show  "result \<in> result_maggaux \<lparr>aggargs_cols = cols, aggargs_n = n, aggargs_g0 = g0, aggargs_y = y, aggargs_\<omega> = \<omega>, aggargs_b = b, aggargs_f = f\<rparr> (SumAux m)"
         using key_in_map False by auto
     qed
   qed
 qed
 next 
-  case(MinAux x)
-  then show ?case by auto
-next
-  case(MaxAux x)
-  then show ?case by auto
-next  
-  case(MedAux x)
-  then show ?case by auto
+  case(RankAux m)
+  then show ?case sorry
 next
   case(CntAux m)
   have agg_type: "fst \<omega> = Formula.Agg_Cnt" using CntAux by auto
@@ -1105,13 +1796,13 @@ next
       define M where [simp]: "M = (\<lambda>y. (y, ecard (Set.filter (\<lambda>x. meval_trm f x = y) group))) ` meval_trm f ` group"
       have "Mapping.lookup m k = Some (length (flatten_multiset M))" 
         using CntAux k_assm 
-        by (simp add: Let_def lookup_default_def)
+        by (simp add: lookup_default_def)
       then have "result = k[y:= Some (eval_agg_op \<omega> M)]" 
         using k_assm agg_type 
         by (metis eval_agg_op.simps(1) option.simps(5) prod.collapse)
       then show "result \<in> eval_aggargs \<lparr>aggargs_cols = cols, aggargs_n = n, aggargs_g0 = g0, aggargs_y = y, aggargs_\<omega> = \<omega>, aggargs_b = b, aggargs_f = f\<rparr> X"
         using k_assm CntAux
-        by (auto simp add: Let_def eval_agg_def eval_aggargs_def)
+        by (auto simp add: eval_agg_def eval_aggargs_def)
     next
       fix result
       assume "result \<in> eval_aggargs \<lparr>aggargs_cols = cols, aggargs_n = n, aggargs_g0 = g0, aggargs_y = y, aggargs_\<omega> = \<omega>, aggargs_b = b, aggargs_f = f\<rparr> X"
@@ -1127,7 +1818,7 @@ next
       define M where [simp]: "M = (\<lambda>y. (y, ecard (Set.filter (\<lambda>x. meval_trm f x = y) group))) ` meval_trm f ` group"
       have "Mapping.lookup m k = Some (length (flatten_multiset M))"
         using CntAux k_assm
-        by (simp add: Let_def lookup_default_def)
+        by (simp add: lookup_default_def)
       then have "result = (case Mapping.lookup m k of
                              Some i \<Rightarrow> k[y:=Some (EInt (integer_of_int i))]
                            | None \<Rightarrow> k)"
@@ -1140,7 +1831,10 @@ next
   qed
 qed
 
-lemma valid_result_maggaux: "valid_maggaux args aux X \<Longrightarrow> result_maggaux args aux = eval_aggargs args X"
+lemma valid_result_maggaux': "valid_maggaux args aux X \<Longrightarrow> result_maggaux args aux = eval_aggargs args X"
   using valid_result_maggaux_unfolded by (cases args) fast
+
+interpretation maggaux valid_maggaux init_maggaux insert_maggaux delete_maggaux result_maggaux
+  using valid_init_maggaux' valid_insert_maggaux' valid_delete_maggaux' valid_result_maggaux' by unfold_locales auto
 
 end
